Sdeque formatting

Sdeque/core.ml
@@ -1,6 +1,10 @@
 open Color.GYR
 
-(** A type for colored buffers. *)
+(* +------------------------------------------------------------------------+ *)
+(* |                                 Types                                  | *)
+(* +------------------------------------------------------------------------+ *)
+
+(** A type for buffers. *)
 type ('a, 'color) buffer =
   | B0 :                           ('a, red            ) buffer
   | B1 : 'a                     -> ('a, nogreen * _ * _) buffer
@@ -9,32 +13,48 @@ type ('a, 'color) buffer =
   | B4 : 'a * 'a * 'a * 'a      -> ('a, nogreen * _ * _) buffer
   | B5 : 'a * 'a * 'a * 'a * 'a -> ('a, red            ) buffer
 
-  (** A type for packets. *)
+(** A type for packets. *)
 type ('a, 'b, 'color) packet =
-  (* The empty packet. *)
   | Hole : ('a, 'a, uncolored) packet
   | Packet : ('a, 'c) buffer
            * ('a * 'a, 'b, nogreen * _ * nored) packet
            * ('a, 'c) buffer
           -> ('a, 'b, 'c) packet
 
+(** A type for the regularity relation. *)
 type ('color_pkt, 'color_chain) regularity =
   | G : (green , _ * noyellow * _) regularity
   | Y : (yellow, green) regularity
   | R : (red   , green) regularity
 
-(** A typed for colored deques. *)
+(** A typed for chains. *)
 type ('a, 'color) chain =
-  (* Colored deque made of only one buffer. *)
   | Ending : ('a, _) buffer -> ('a, green) chain
+  | Chain :  ('c1, 'c2) regularity * ('a, 'b, 'c1) packet * ('b, 'c2) chain
+          -> ('a, 'c1) chain
 
-  | Chain : ('c1, 'c2) regularity
-          * ('a, 'b, 'c1) packet
-          * ('b, 'c2) chain
-         -> ('a, 'c1) chain
+(** A type decomposing buffers according to their number of elements.
+    Buffers with 0 or 1 element are decomposed into [Underflow];
+    buffers with 2 or 3 elements are decomposed into [Ok];
+    buffers with 4 or 5 elements are decomposed into [Overflow]. *)
+type 'a decompose =
+  | Underflow : 'a option -> 'a decompose
+  | Ok        : ('a, green) buffer -> 'a decompose
+  | Overflow  : ('a, green) buffer * ('a * 'a) -> 'a decompose
+
+(** A type decomposing a buffer into its first element, a central buffer, and
+    its last element. If such a decomposition is not possible, an option
+    representing the buffer is returned with [Alone]. *)
+type 'a sandwich =
+  | Alone    : 'a option                -> 'a sandwich
+  | Sandwich : 'a * ('a, _) buffer * 'a -> 'a sandwich
 
 (** A type for deques. *)
 type 'a deque = T : ('a, _ * _ * nored) chain -> 'a deque
+
+(* +------------------------------------------------------------------------+ *)
+(* |                                 Empty                                  | *)
+(* +------------------------------------------------------------------------+ *)
 
 (** The empty deque. *)
 let empty = T (Ending B0)
@@ -42,10 +62,78 @@ let empty = T (Ending B0)
 (** Emptyness test for deques. *)
 let is_empty d = d = empty
 
-(** Pushes an element onto a buffer, and returns a green chain. *)
-let buffer_push : type a c. a -> (a, c) buffer -> (a, green) chain
+(* +------------------------------------------------------------------------+ *)
+(* |                                  Core                                  | *)
+(* +------------------------------------------------------------------------+ *)
+
+(** Pushes on a green buffer. *)
+let green_push
+: type a. a -> (a, green) buffer -> (a, yellow) buffer
 = fun x buf ->
   match buf with
+  | B2 (a, b)    -> B3 (x, a, b)
+  | B3 (a, b, c) -> B4 (x, a, b, c)
+
+(** Injects on a green buffer. *)
+let green_inject
+: type a. (a, green) buffer -> a -> (a, yellow) buffer
+= fun buf x ->
+  match buf with
+  | B2 (a, b)    -> B3 (a, b, x)
+  | B3 (a, b, c) -> B4 (a, b, c, x)
+
+(** Pops off a green buffer. *)
+let green_pop : type a. (a, green) buffer -> a * (a, yellow) buffer
+= function
+  | B2 (a, b)    -> a, B1 b
+  | B3 (a, b, c) -> a, B2 (b, c)
+
+(** Ejects off a green buffer. *)
+let green_eject : type a. (a, green) buffer -> (a, yellow) buffer * a
+= function
+  | B2 (a, b)    -> B1 a, b
+  | B3 (a, b, c) -> B2 (a, b), c
+
+(** Pushes on a yellow buffer. *)
+let yellow_push : type a. a -> (a, yellow) buffer -> (a, red) buffer
+= fun x b ->
+  match b with
+  | B1 a            -> B2 (x, a)
+  | B2 (a, b)       -> B3 (x, a, b)
+  | B3 (a, b, c)    -> B4 (x, a, b, c)
+  | B4 (a, b, c, d) -> B5 (x, a, b, c, d)
+
+(** Injects on a yellow buffer. *)
+let yellow_inject : type a. (a, yellow) buffer -> a -> (a, red) buffer
+= fun b x ->
+  match b with
+  | B1 a            -> B2 (a, x)
+  | B2 (a, b)       -> B3 (a, b, x)
+  | B3 (a, b, c)    -> B4 (a, b, c, x)
+  | B4 (a, b, c, d) -> B5 (a, b, c, d, x)
+
+(** Pops off a yellow buffer. *)
+let yellow_pop : type a. (a, yellow) buffer -> a * (a, red) buffer
+= fun b ->
+  match b with
+  | B1 a            -> a, B0
+  | B2 (a, b)       -> a, (B1  b)
+  | B3 (a, b, c)    -> a, (B2 (b, c))
+  | B4 (a, b, c, d) -> a, (B3 (b, c, d))
+
+(** Ejects off a yellow buffer. *)
+let yellow_eject : type a. (a, yellow) buffer -> (a, red) buffer * a
+= fun b ->
+  match b with
+  | B1 a            -> B0,             a
+  | B2 (a, b)       -> (B1  a),        b
+  | B3 (a, b, c)    -> (B2 (a, b)),    c
+  | B4 (a, b, c, d) -> (B3 (a, b, c)), d
+
+(** Pushes on a buffer, and returns a green chain. *)
+let buffer_push : type a c. a -> (a, c) buffer -> (a, green) chain
+= fun x b ->
+  match b with
   | B0 -> Ending (B1 x)
   | B1 a -> Ending (B2 (x, a))
   | B2 (a, b) -> Ending (B3 (x, a, b))
@@ -54,10 +142,10 @@ let buffer_push : type a c. a -> (a, c) buffer -> (a, green) chain
   | B5 (a, b, c, d, e) ->
       Chain (G, Packet (B3 (x, a, b), Hole, B3 (c, d, e)), Ending B0)
 
-(** Injects an element onto a buffer, and returns a green chain. *)
+(** Injects on a buffer, and returns a green chain. *)
 let buffer_inject : type a c. (a, c) buffer -> a -> (a, green) chain
-= fun buf x ->
-  match buf with
+= fun b x ->
+  match b with
   | B0 -> Ending (B1 x)
   | B1 a -> Ending (B2 (a, x))
   | B2 (a, b) -> Ending (B3 (a, b, x))
@@ -66,161 +154,64 @@ let buffer_inject : type a c. (a, c) buffer -> a -> (a, green) chain
   | B5 (a, b, c, d, e) ->
       Chain (G, Packet (B3 (a, b, c), Hole, B3 (d, e, x)), Ending B0)
 
-(** Pops an element from a buffer, when there is no elements in the buffer, an
-    error is raised. Otherwise, it returns the removed element and the new
-    buffer. *)
-let buffer_pop_unsafe : type a c. (a, c) buffer -> a * (a, red) buffer
-= function
-  | B0 -> assert false
-  | B1 a -> a, B0
-  | B2 (a, b) -> a, (B1 b)
-  | B3 (a, b, c) -> a, (B2 (b, c))
-  | B4 (a, b, c, d) -> a, (B3 (b, c, d))
-  | B5 (a, b, c, d, e) -> a, (B4 (b, c, d, e))
-
-(** Pops an element from a buffer, if the buffer is empty, it returns [None],
-    otherwise, it returns an option containing the removed element and the new
-    buffer. *)
+(** Pops off a buffer, and returns an option. *)
 let buffer_pop : type a c. (a, c) buffer -> (a * (a, red) buffer) option
 = function
-  | B0  -> None
-  | buf -> Some (buffer_pop_unsafe buf)
+  | B0 -> None
+  | B1 a -> Some (a, B0)
+  | B2 (a, b) -> Some (a, (B1 b))
+  | B3 (a, b, c) -> Some (a, (B2 (b, c)))
+  | B4 (a, b, c, d) -> Some (a, (B3 (b, c, d)))
+  | B5 (a, b, c, d, e) -> Some (a, (B4 (b, c, d, e)))
 
-(** Ejects an element from a buffer, when there is no elements in the buffer, an
-    error is raised. Otherwise, it returns the new buffer and the removed
-    element. *)
-let buffer_eject_unsafe : type a c. (a, c) buffer -> (a, red) buffer * a
-= function
-  | B0 -> assert false
-  | B1 a -> B0, a
-  | B2 (a, b) -> (B1 a), b
-  | B3 (a, b, c) -> (B2 (a, b)), c
-  | B4 (a, b, c, d) -> (B3 (a, b, c)), d
-  | B5 (a, b, c, d, e) -> (B4 (a, b, c, d)), e
-
-(** Ejects an element from a buffer, if the buffer is empty, it returns [None],
-    otherwise, it returns an option containing the removed element and the new
-    buffer. *)
+(** Ejects off a buffer, and returns an option. *)
 let buffer_eject : type a c. (a, c) buffer -> ((a, red) buffer * a) option
 = function
-  | B0  -> None
-  | buf -> Some (buffer_eject_unsafe buf)
+  | B0 -> None
+  | B1 a -> Some (B0, a)
+  | B2 (a, b) -> Some ((B1 a), b)
+  | B3 (a, b, c) -> Some ((B2 (a, b)), c)
+  | B4 (a, b, c, d) -> Some ((B3 (a, b, c)), d)
+  | B5 (a, b, c, d, e) -> Some ((B4 (a, b, c, d)), e)
 
-(** Pushes an element onto a green buffer, returning a yellow one. *)
-let green_push
-: type a. a -> (a, green) buffer -> (a, yellow) buffer
-= fun x buf ->
-  match buf with
-  | B2 (a, b) -> B3 (x, a, b)
-  | B3 (a, b, c) -> B4 (x, a, b, c)
-
-(** Injects an element onto a green buffer, returning a yellow one. *)
-let green_inject
-: type a. (a, green) buffer -> a -> (a, yellow) buffer
-= fun buf x ->
-  match buf with
-  | B2 (a, b)    -> B3 (a, b, x)
-  | B3 (a, b, c) -> B4 (a, b, c, x)
-
-(** Pops an element from a green buffer, returns the removed element and the
-    new yellow buffer. *)
-let green_pop : type a. (a, green) buffer -> a * (a, yellow) buffer
-= function
-  | B2 (a, b)    -> a, B1 b
-  | B3 (a, b, c) -> a, B2 (b, c)
-
-(** Ejects an element from a green buffer, returns the new yellow buffer and
-    the removed element. *)
-let green_eject : type a. (a, green) buffer -> (a, yellow) buffer * a
-= function
-  | B2 (a, b)    -> B1 a, b
-  | B3 (a, b, c) -> B2 (a, b), c
-
-(** Pushes an element onto a yellow buffer, and returns the new buffer. *)
-let yellow_push : type a. a -> (a, yellow) buffer -> (a, red) buffer
-= fun x buf ->
-  match buf with
-  | B1 a -> B2 (x, a)
-  | B2 (a, b) -> B3 (x, a, b)
-  | B3 (a, b, c) -> B4 (x, a, b, c)
-  | B4 (a, b, c, d) -> B5 (x, a, b, c, d)
-
-(** Injects an element onto a yellow buffer, and returns the new buffer. *)
-let yellow_inject : type a. (a, yellow) buffer -> a -> (a, red) buffer
-= fun buf x ->
-  match buf with
-  | B1 a -> B2 (a, x)
-  | B2 (a, b) -> B3 (a, b, x)
-  | B3 (a, b, c) -> B4 (a, b, c, x)
-  | B4 (a, b, c, d) -> B5 (a, b, c, d, x)
-
-(** Pops an element from a yellow buffer, returns the removed element and the
-    new buffer. *)
-let yellow_pop : type a. (a, yellow) buffer -> a * (a, red) buffer
-= fun buf ->
-  match buf with
-  | B1 a            -> a, B0
-  | B2 (a, b)       -> a, (B1  b)
-  | B3 (a, b, c)    -> a, (B2 (b, c))
-  | B4 (a, b, c, d) -> a, (B3 (b, c, d))
-
-(** Ejects an element from a yellow buffer, returns the new buffer and the
-    removed element. *)
-let yellow_eject : type a. (a, yellow) buffer -> (a, red) buffer * a
-= fun buf ->
-  match buf with
-  | B1 a            -> B0,             a
-  | B2 (a, b)       -> (B1  a),        b
-  | B3 (a, b, c)    -> (B2 (a, b)),    c
-  | B4 (a, b, c, d) -> (B3 (a, b, c)), d
-
-(** Performs a push then an eject. *)
+(** Pushes then ejects. *)
 let prefix_rot : type a c. a -> (a, c) buffer -> (a, c) buffer * a
 = fun x buf -> match buf with
-  | B0                 -> B0, x
-  | B1 a               -> B1  x, a
-  | B2 (a, b)          -> B2 (x, a), b
-  | B3 (a, b, c)       -> B3 (x, a, b), c
-  | B4 (a, b, c, d)    -> B4 (x, a, b, c), d
+  | B0 -> B0, x
+  | B1 a -> B1  x, a
+  | B2 (a, b) -> B2 (x, a), b
+  | B3 (a, b, c) -> B3 (x, a, b), c
+  | B4 (a, b, c, d) -> B4 (x, a, b, c), d
   | B5 (a, b, c, d, e) -> B5 (x, a, b, c, d), e
 
-(** Performs an inject then a pop. *)
+(** Injects then pops. *)
 let suffix_rot : type a c. (a, c) buffer -> a -> a * (a, c) buffer
 = fun buf x -> match buf with
-  | B0                 -> x, B0
-  | B1 a               -> a, B1 x
-  | B2 (a, b)          -> a, B2 (b, x)
-  | B3 (a, b, c)       -> a, B3 (b, c, x)
-  | B4 (a, b, c, d)    -> a, B4 (b, c, d, x)
+  | B0 -> x, B0
+  | B1 a -> a, B1 x
+  | B2 (a, b) -> a, B2 (b, x)
+  | B3 (a, b, c) -> a, B3 (b, c, x)
+  | B4 (a, b, c, d) -> a, B4 (b, c, d, x)
   | B5 (a, b, c, d, e) -> a, B5 (b, c, d, e, x)
 
-(** Create a green buffer by injecting a pair onto an option.*)
+(** Merges an option and a pair to create a green buffer. *)
 let prefix23 opt (b, c) = match opt with
   | None   -> B2 (b, c)
   | Some a -> B3 (a, b, c)
 
-(** Create a green buffer by pushing a pair onto an option. *)
+(** Merges a pair and an option to create a green buffer. *)
 let suffix23 (a, b) opt = match opt with
   | None   -> B2 (a, b)
   | Some c -> B3 (a, b, c)
 
-(** Create a yellow (or green) buffer by pushing an element onto an option. *)
-let suffix12 x opt = match opt with
+(** Merges an element and an option to create a yellow buffer. *)
+let prefix12 x opt = match opt with
   | None   -> B1 x
   | Some y -> B2 (x, y)
 
-(** Type ['a decompose] helps us describe a 'a buffer. A buffer with 0 or 1
-    elements is considered [Underflow], it cannot be green unless we add
-    elements. If the buffer is green, it's [Ok]. And if the buffer has 4 or 5
-    elements, the buffer [Overflow], we can make it green by removing a pair. *)
-type 'a decompose =
-  | Underflow : 'a option -> 'a decompose
-  | Ok        : ('a, green) buffer -> 'a decompose
-  | Overflow  : ('a, green) buffer * ('a * 'a) -> 'a decompose
-
 (** Returns the decomposed version of a buffer. Here, it is a prefix
-    decomposition: when the buffer is overflowed, elements at the end are
-    removed. *)
+    decomposition: when the buffer has 4 or 5 elements, those at the end are
+    set appart. *)
 let prefix_decompose : type a c. (a, c) buffer -> a decompose
 = function
   (* No element, the buffer is underflowed. *)
@@ -236,8 +227,8 @@ let prefix_decompose : type a c. (a, c) buffer -> a decompose
   | B5 (a, b, c, d, e) -> Overflow (B3 (a, b, c), (d, e))
 
 (** Returns the decomposed version of a buffer. Here, it is a suffix
-    decomposition: when the buffer is overflowed, elements at the beginning are
-    removed. *)
+    decomposition: when the buffer has 4 or 5 elements, those at the start are
+    set appart. *)
 let suffix_decompose : type a c. (a, c) buffer -> a decompose
 = function
   (* No element, the buffer is underflowed. *)
@@ -252,16 +243,7 @@ let suffix_decompose : type a c. (a, c) buffer -> a decompose
   | B4 (a, b, c, d)    -> Overflow (B2 (c, d), (a, b))
   | B5 (a, b, c, d, e) -> Overflow (B3 (c, d, e), (a, b))
 
-
-(** Type ['a sandwich] helps us to represent a 'a buffer. If a buffer contains
-    0 or 1 element, then it is considered alone and can be represented by an
-    option type. If it has more elements, we can represent our buffer by a
-    smaller one sandwiched between two elements. *)
-type 'a sandwich =
-  | Alone : 'a option -> 'a sandwich
-  | Sandwich : 'a * ('a, _) buffer * 'a -> 'a sandwich
-
-(** Returns the sandwich representation of a buffer. *)
+(** Returns the sandwiched version of a buffer. *)
 let buffer_unsandwich : type a c. (a, c) buffer -> a sandwich
 = function
   | B0 -> Alone None
@@ -271,18 +253,18 @@ let buffer_unsandwich : type a c. (a, c) buffer -> a sandwich
   | B4 (a, b, c, d) -> Sandwich (a, B2 (b, c), d)
   | B5 (a, b, c, d, e) -> Sandwich (a, B3 (b, c, d), e)
 
-(** Translates a 'a buffer to a 'a * 'a buffer. A additional option type is
-    returned to handle cases where the buffer contains an odd number of
-    elements. *)
+(** Converts a buffer to a buffer of pairs. If the buffer has an odd number of
+    elements, the first is returned via an option. *)
 let buffer_halve : type a c. (a, c) buffer -> a option * (a * a, red) buffer
 = function
-  | B0                 -> None,   B0
-  | B1 a               -> Some a, B0
-  | B2 (a, b)          -> None,   (B1 (a, b))
-  | B3 (a, b, c)       -> Some a, (B1 (b, c))
-  | B4 (a, b, c, d)    -> None,   (B2 ((a, b), (c, d)))
-  | B5 (a, b, c, d, e) -> Some a, (B2 ((b, c), (d, e)))
+  | B0 -> None, B0
+  | B1 a -> Some a, B0
+  | B2 (a, b) -> None, B1 (a, b)
+  | B3 (a, b, c) -> Some a, B1 (b, c)
+  | B4 (a, b, c, d) -> None, B2 ((a, b), (c, d))
+  | B5 (a, b, c, d, e) -> Some a, B2 ((b, c), (d, e))
 
+(** Makes a non-red buffer yellow. *)
 let to_yellow : type a g y. (a, g * y * nored) buffer -> (a, yellow) buffer
 = function
   | B1 a -> B1 a
@@ -290,6 +272,7 @@ let to_yellow : type a g y. (a, g * y * nored) buffer -> (a, yellow) buffer
   | B3 (a, b, c) -> B3 (a, b, c)
   | B4 (a, b, c, d) -> B4 (a, b, c, d)
 
+(** Makes a buffer of any color red. *)
 let to_red : type a c. (a, c) buffer -> (a, red) buffer
 = function
   | B0 -> B0
@@ -299,256 +282,235 @@ let to_red : type a c. (a, c) buffer -> (a, red) buffer
   | B4 (a, b, c, d) -> B4 (a, b, c, d)
   | B5 (a, b, c, d, e) -> B5 (a, b, c, d, e)
 
-(** Takes any 'a buffer and a green ('a * 'a) one, and rearranges elements
-    contained in the two buffers to return one green 'a buffer and a yellow
-    ('a * 'a) buffer. The order of elements is preserved. *)
+(** Takes a buffer of any color and a green buffer of pairs, rearranges elements
+    contained in them, and returns a green buffer and a yellow buffer of pairs.
+    The order of elements is preserved. *)
 let green_prefix_concat
 : type a c.
-      (a, c) buffer
+     (a, c) buffer
   -> (a * a, green) buffer
   -> (a, green) buffer * ((a * a), yellow) buffer
-= fun buf1 buf2 ->
-  match prefix_decompose buf1 with
-  (* If the first one is already green, we have nothing to do. *)
-  | Ok buf1 -> buf1, to_yellow buf2
+= fun b1 b2 ->
+  match prefix_decompose b1 with
   (* If the first buffer lacks elements, we pop a pair from the second one and
       inject it onto the first one. *)
   | Underflow opt ->
-      let ab, buf2 = green_pop buf2 in
-      prefix23 opt ab, buf2
+      let ab, b2 = green_pop b2 in
+      prefix23 opt ab, b2
+  (* If the first buffer is already green, we have nothing to do. *)
+  | Ok b1 -> b1, to_yellow b2
   (* If the first buffer has to much elements, we simply push them onto the
       second one. *)
-  | Overflow (buf1, ab) ->
-      buf1, green_push ab buf2
+  | Overflow (b1, ab) -> b1, green_push ab b2
 
-(** Takes a ('a * 'a) green buffer and any 'a one, and rearranges elements
-    contained in the two buffers to return one ('a * 'a) yellow buffer and one
-    green 'a buffer. The order of elements is preserved. *)
+(** Takes a green buffer of pairs and a buffer of any color, rearranges elements
+    contained in them, and returns a yellow buffer of pairs and a green buffer.
+    The order of elements is preserved. *)
 let green_suffix_concat
 : type a c.
       (a * a, green) buffer
   -> (a, c) buffer
   -> ((a * a), yellow) buffer * (a, green) buffer
-= fun buf1 buf2 ->
-  match suffix_decompose buf2 with
-  | Ok buf2 -> to_yellow buf1, buf2
+= fun b1 b2 ->
+  match suffix_decompose b2 with
   | Underflow opt ->
-      let buf1, ab = green_eject buf1 in
-      buf1, suffix23 ab opt
-  | Overflow (buf2, ab) ->
-      green_inject buf1 ab, buf2
+      let b1, ab = green_eject b1 in
+      b1, suffix23 ab opt
+  | Ok b2 -> to_yellow b1, b2
+  | Overflow (b2, ab) -> green_inject b1 ab, b2
 
-(** Takes any 'a buffer and a yellow ('a * 'a) one, and rearranges elements
-    contained in the two buffers to return one green 'a buffer and any ('a * 'a)
-    buffer. The order of elements is preserved. *)
-let prefix_concat buf1 buf2 =
-  match prefix_decompose buf1 with
-  (* If the first one is already green, we have nothing to do. *)
-  | Ok buf1 ->
-      buf1, to_red buf2
+(** Takes a buffer of any color and a yellow buffer of pairs, rearranges
+    elements contained in them, and returns a green buffer and a buffer of pairs
+    of any color.
+    The order of elements is preserved. *)
+let prefix_concat b1 b2 =
+  match prefix_decompose b1 with
   (* If the first buffer lacks elements, we pop a pair from the second one and
       inject it onto the first one. *)
   | Underflow opt ->
-      let ab, buf2 = yellow_pop buf2 in
-      prefix23 opt ab, buf2
+      let ab, b2 = yellow_pop b2 in
+      prefix23 opt ab, b2
+  (* If the first one is already green, we have nothing to do. *)
+  | Ok b1 -> b1, to_red b2
   (* If the first buffer has to much elements, we simply push them onto the
       second one. *)
-  | Overflow (buf1, ab) ->
-      buf1, yellow_push ab buf2
+  | Overflow (b1, ab) -> b1, yellow_push ab b2
 
-(** Takes a yellow ('a * 'a) buffer and any 'a one, and rearranges elements
-    contained in the two buffers to return any ('a * 'a) buffer and one green
-    'a buffer. The order of elements is preserved. *)
-let suffix_concat buf1 buf2 =
+(** Takes a yellow buffer of pairs and a buffer of any color, rearranges
+    elements contained in them, and returns a buffer of pairs of any color and a
+    green buffer.
+    The order of elements is preserved. *)
+let suffix_concat b1 b2 =
   (* The reasoning is the same as in the previous case. *)
-  match suffix_decompose buf2 with
-  | Ok buf2 ->
-      to_red buf1, buf2
+  match suffix_decompose b2 with
   | Underflow opt ->
-      let buf1, ab = yellow_eject buf1 in
-      buf1, suffix23 ab opt
-  | Overflow (buf2, ab) ->
-      yellow_inject buf1 ab, buf2
+      let b1, ab = yellow_eject b1 in
+      b1, suffix23 ab opt
+  | Ok b2 -> to_red b1, b2
+  | Overflow (b2, ab) -> yellow_inject b1 ab, b2
 
-(** Takes a prefix buffer, a following buffer (when the next level is composed
-    of only one buffer), and a suffix buffer. It allows to rearrange all
-    elements contained in those buffers into a green chain. *)
+(** Takes a prefix buffer, a child buffer, and a suffix buffer, and rearranges
+    all elements contained in these buffers to form a green chain.
+    The order of elements is preserved. *)
 let make_small
-= fun prefix1 buf suffix1 ->
-  match prefix_decompose prefix1, suffix_decompose suffix1 with
-  (* If the prefix and suffix are green, no changes are needed. In practice, this case
-      never occurs as we call the function on a red buffer. *)
-  | Ok p1, Ok s1 ->
-      Chain (G, Packet (p1, Hole, s1), Ending buf)
-
-  (* Only the prefix is green. *)
-  | Ok p1, Underflow opt ->
-      begin match buffer_eject buf, opt with
-      (* The suffix and the following buffer are empty. We can return a chain
-          containing only the prefix. *)
-      | None, None   -> Ending p1
-      (* If the suffix contains one element and the following buffer is empty.
-          We simply inject this element in p1. In practice, this case never
-          occurs as we call the function on a red buffer. If the prefix is green,
-          the suffix must be red, as it is underflowed it is empty. *)
-      | None, Some x -> buffer_inject p1 x
-      (* If the following buffer is not empty, we can eject elements from it
-          and push them onto our suffix. *)
-      | Some (rest, cd), _ ->
-          Chain (G, Packet (p1, Hole, suffix23 cd opt), Ending rest)
-      end
-
-  (* Only the suffix is green. This is symmetrical to the previous case. *)
-  | Underflow opt, Ok s1 ->
-      begin match buffer_pop buf, opt with
-      | None, None   -> Ending s1
-      | None, Some x -> buffer_push x s1
-      | Some (cd, rest), _ ->
-          Chain (G, Packet (prefix23 opt cd, Hole, s1), Ending rest)
-      end
-
+= fun b1 b2 b3 ->
+  match prefix_decompose b1, suffix_decompose b3 with
   (* Both the prefix and the suffix are underflowed. *)
   | Underflow p1, Underflow s1 ->
-      begin match buffer_unsandwich buf with
-      (* If the following buffer has enough elements to be sandwich, we can
-          use the sandwiching elements and inject/push them onto our prefix/
-          suffix. *)
-      | Sandwich (ab, rest, cd) ->
-          Chain (G, Packet (prefix23 p1 ab, Hole, suffix23 cd s1), Ending rest)
-      (* We don't have enough elements in our following buffer, we have to
-          treat our result case by case. It correspond to the "No-Buffer Case"
-          from Kaplan and Tarjan's paper. *)
-      | Alone opt ->
-          begin match p1, opt, s1 with
-          | None,   None,        None   -> Ending B0
-          | Some a, None,        None
-          | None,   None,        Some a -> Ending (B1 a)
-          | Some a, None,        Some b
-          | None,   Some (a, b), None   -> Ending (B2 (a, b))
-          | Some a, Some (b, c), None
-          | None,   Some (a, b), Some c -> Ending (B3 (a, b, c))
-          | Some a, Some (b, c), Some d -> Ending (B4 (a, b, c, d))
-          end
+    begin match buffer_unsandwich b2 with
+    (* If the child buffer has 0 or 1 element, an ending chain is constructed
+       containing all elements. *)
+    | Alone opt ->
+      begin match p1, opt, s1 with
+      | None,   None,        None   -> Ending B0
+      | Some a, None,        None
+      | None,   None,        Some a -> Ending (B1 a)
+      | Some a, None,        Some b
+      | None,   Some (a, b), None   -> Ending (B2 (a, b))
+      | Some a, Some (b, c), None
+      | None,   Some (a, b), Some c -> Ending (B3 (a, b, c))
+      | Some a, Some (b, c), Some d -> Ending (B4 (a, b, c, d))
       end
+    (* If the child buffer has more than 2 elements, it can be sandwiched, and
+       green prefix and suffix buffers are constructed. *)
+    | Sandwich (ab, rest, cd) ->
+        Chain (G, Packet (prefix23 p1 ab, Hole, suffix23 cd s1), Ending rest)
+    end
 
-  (* If we have an overflowing prefix and a good suffix, we can simply push its
-      excess elements onto the following buffer. *)
-  | Overflow (p1, ab), Ok s1 ->
-      let buf = buffer_push ab buf in
-      Chain (G, Packet (p1, Hole, s1), buf)
+  (* Only the prefix is underflowed. *)
+  | Underflow p1, Ok s1 ->
+    begin match buffer_pop b2, p1 with
+    (* If the child buffer has 0 element, elements from the prefix are pushed
+       on the suffix to make an ending chain. *)
+    | None, None   -> Ending s1
+    | None, Some x -> buffer_push x s1
+    (* If the child buffer has more than 1 element, this element is poped and
+       added to the prefix to make it green. *)
+    | Some (cd, rest), _ ->
+        Chain (G, Packet (prefix23 p1 cd, Hole, s1), Ending rest)
+    end
 
-  (* This is symmetrical to the previous case. *)
+  (* The prefix is underflowed, the suffix is overflowed. *)
+  | Underflow p1, Overflow (s1, ab) ->
+      let cd, center = suffix_rot b2 ab in
+      Chain (G, Packet (prefix23 p1 cd, Hole, s1), Ending center)
+
+  (* Only the suffix is underflowed. Similar to the symmetric case. *)
+  | Ok p1, Underflow s1 ->
+    begin match buffer_eject b2, s1 with
+    | None, None   -> Ending p1
+    | None, Some x -> buffer_inject p1 x
+    | Some (rest, ab), _ ->
+        Chain (G, Packet (p1, Hole, suffix23 ab s1), Ending rest)
+    end
+
+  (* Both the prefix and the suffix are green. *)
+  | Ok p1, Ok s1 -> Chain (G, Packet (p1, Hole, s1), Ending b2)
+
+  (* Only the suffix is overflowed. *)
   | Ok p1, Overflow (s1, ab) ->
-      let buf = buffer_inject buf ab in
-      Chain (G, Packet (p1, Hole, s1), buf)
+      (* Excess elements are injected in the child buffer. *)
+      let c2 = buffer_inject b2 ab in
+      Chain (G, Packet (p1, Hole, s1), c2)
 
-  (* If the prefix is underflowing and the suffix overflowing, we add the
-      suffix's excess elements to the following buffer, and retrieve its first
-    pair. This pair can be added to the prefix to make it green. *)
-  | Underflow opt, Overflow (s1, ab) ->
-      let cd, center = suffix_rot buf ab in
-      Chain (G, Packet (prefix23 opt cd, Hole, s1), Ending center)
+  (* The prefix is overflowed, the suffix is underflowed. Similar to the
+     symmetric case. *)
+  | Overflow (p1, cd), Underflow s1 ->
+      let center, ab = prefix_rot cd b2 in
+      Chain (G, Packet (p1, Hole, suffix23 ab s1), Ending center)
 
-  (* This is symmetrical to the previous case. *)
-  | Overflow (p1, ab), Underflow opt ->
-      let center, cd = prefix_rot ab buf in
-      Chain (G, Packet (p1, Hole, suffix23 cd opt), Ending center)
+  (* Only the prefix is overflowed. Similar to the symmetric case. *)
+  | Overflow (p1, cd), Ok s1 ->
+      let c2 = buffer_push cd b2 in
+      Chain (G, Packet (p1, Hole, s1), c2)
 
-  (* If both the prefix and the suffix are overflowing, a new level is added,
-      all excess elements can be stored in a yellow packet. *)
-  | Overflow (p1, ab), Overflow (s1, cd) ->
-      let x, rest = buffer_halve buf in
-      let p2 = suffix12 ab x in
-      Chain (G, Packet (p1, Packet (p2, Hole, B1 cd), s1), Ending rest)
+  (* Both the prefix and the suffix are overflowed. *)
+  | Overflow (p1, cd), Overflow (s1, ab) ->
+    let x, rest = buffer_halve b2 in
+    let p2 = prefix12 cd x in
+      Chain (G, Packet (p1, Packet (p2, Hole, B1 ab), s1), Ending rest)
 
-(** Takes a red chain and returns a green one representing the same set. *)
+(** Makes a red chain green. *)
 let green_of_red
 : type a. (a, red) chain -> (a, green) chain
 = function
-  (* If our red packet is at the end of the chain, we handle a lot of different
-      cases in the make_small function. *)
+  (* If the red node comes just before the ending, a lot of different cases are
+     handled by [make_small]. *)
   | Chain (R, Packet (p1, Hole, s1), Ending buf) ->
       make_small p1 buf s1
-  (* If our red packet is followed by a yellow one, we are in the "Two-Buffer
-      Case" from Kaplan and Tarjan's paper. *)
-  | Chain (R, Packet (p1, Packet (p2, child, s2), s1), chain) ->
-      let p1, p2 = prefix_concat p1 (to_yellow p2) in
-      let s2, s1 = suffix_concat (to_yellow s2) s1 in
-      Chain (G, Packet (p1, Hole, s1), Chain (R, Packet (p2, child, s2), chain))
-  (* If our red packet is followed by a green one, we are in the "Two-Buffer
-      Case" from Kaplan and Tarjan's paper. *)
-  | Chain (R, Packet (p1, Hole, s1), Chain (G, Packet (p2, child, s2), chain)) ->
+  (* Otherwise, the prefix and suffix of the following node are used to make
+     the prefix and the suffix of the red node green. *)
+  | Chain (R, Packet (p1, Hole, s1), Chain (G, Packet (p2, child, s2), c)) ->
       let p1, p2 = green_prefix_concat p1 p2 in
       let s2, s1 = green_suffix_concat s2 s1 in
-      Chain (G, Packet (p1, Packet (p2, child, s2), s1), chain)
+      Chain (G, Packet (p1, Packet (p2, child, s2), s1), c)
+  | Chain (R, Packet (p1, Packet (p2, child, s2), s1), c) ->
+      let p1, p2 = prefix_concat p1 (to_yellow p2) in
+      let s2, s1 = suffix_concat (to_yellow s2) s1 in
+      Chain (G, Packet (p1, Hole, s1), Chain (R, Packet (p2, child, s2), c))
 
-(** Takes a green or red chain, and returns a green one representing
-    the same set. *)
+(** Makes a green or red chain green. *)
 let ensure_green
 : type a g r. (a, g * noyellow * r) chain -> (a, green) chain
 = function
-  | Ending buf -> Ending buf
-  | Chain (G, x, k) -> Chain (G, x, k)
-  | Chain (R, x, k) -> green_of_red (Chain (R, x, k))
+  | Ending b          -> Ending b
+  | Chain (G, pkt, c) -> Chain (G, pkt, c)
+  | Chain (R, pkt, c) -> green_of_red (Chain (R, pkt, c))
 
-(** Takes a yellow packet, [p1], [child], [s1], and a chain [chain]. Returns
-    a deque starting with this packet and followed by the green version of
-    [chain]. *)
-let yellow p1 child s1 chain =
-  T (Chain (Y, Packet (to_yellow p1, child, to_yellow s1), ensure_green chain))
+(** Takes a prefix non-red buffer, a child packet and a suffix non-red buffer,
+    and a following green or red chain, and makes a deque out of them. *)
+let make_yellow p1 child s1 c =
+  T (Chain (Y, Packet (to_yellow p1, child, to_yellow s1), ensure_green c))
 
-(** Takes a red packet, [p1], [child], [s1], and a green chain [chain].
-    Returns the green version of the chain made of the red packet followed by
-    the green chain. *)
-let red p1 child s1 chain =
-  T (green_of_red (Chain (R, Packet (to_red p1, child, to_red s1), chain)))
+(** Takes a prefix buffer of any color, a child packet and a suffix buffer of
+    any color, and a following green chain, and makes a deque out of them. *)
+let make_red p1 child s1 c =
+  T (green_of_red (Chain (R, Packet (to_red p1, child, to_red s1), c)))
 
-(** Pushes an element on a deque. *)
+(** Pushes on a deque. *)
 let push x (T t) = match t with
-  | Ending buf -> T (buffer_push x buf)
-  | Chain (G, Packet (p1, child, s1), chain) ->
+  | Ending b -> T (buffer_push x b)
+  | Chain (G, Packet (p1, child, s1), c) ->
       let p1 = green_push x p1 in
-      yellow p1 child s1 chain
-  | Chain (Y, Packet (p1, child, s1), chain) ->
+      make_yellow p1 child s1 c
+  | Chain (Y, Packet (p1, child, s1), c) ->
       let p1 = yellow_push x p1 in
-      red p1 child s1 chain
+      make_red p1 child s1 c
 
-(** Injects an element on a deque. *)
+(** Injects on a deque. *)
 let inject (T t) x = match t with
-  | Ending buf -> T (buffer_inject buf x)
-  | Chain (G, Packet (p1, child, s1), chain) ->
+  | Ending b -> T (buffer_inject b x)
+  | Chain (G, Packet (p1, child, s1), c) ->
       let s1 = green_inject s1 x in
-      yellow p1 child s1 chain
-  | Chain (Y, Packet (p1, child, s1), chain) ->
+      make_yellow p1 child s1 c
+  | Chain (Y, Packet (p1, child, s1), c) ->
       let s1 = yellow_inject s1 x in
-      red p1 child s1 chain
+      make_red p1 child s1 c
 
-(** Pops an element from a deque. If the deque is empty, it returns [None], if
-    not, it returns the removed element and the remaining deque. *)
+(** Pops off a deque. *)
 let pop (T t) = match t with
-  | Ending buf ->
-    begin match buffer_pop buf with
+  | Ending b ->
+    begin match buffer_pop b with
     | None -> None
-    | Some (x, buf) -> Some (x, T (Ending buf))
+    | Some (x, b) -> Some (x, T (Ending b))
     end
-  | Chain (G, Packet (p1, child, s1), chain) ->
+  | Chain (G, Packet (p1, child, s1), c) ->
     let x, p1 = green_pop p1 in
-    Some (x, yellow p1 child s1 chain)
-  | Chain (Y, Packet (p1, child, s1), chain) ->
+    Some (x, make_yellow p1 child s1 c)
+  | Chain (Y, Packet (p1, child, s1), c) ->
     let x, p1 = yellow_pop p1 in
-    Some (x, red p1 child s1 chain)
+    Some (x, make_red p1 child s1 c)
 
-(** Ejects an element from a deque. If the deque is empty, it returns [None], if
-    not, it returns the remaining deque and the removed element. *)
+(** Ejects off a deque. *)
 let eject (T t) = match t with
-  | Ending buf ->
-    begin match buffer_eject buf with
+  | Ending b ->
+    begin match buffer_eject b with
     | None -> None
-    | Some (buf, x) -> Some (T (Ending buf), x)
+    | Some (b, x) -> Some (T (Ending b), x)
     end
-  | Chain (G, Packet (p1, child, s1), chain) ->
+  | Chain (G, Packet (p1, child, s1), c) ->
     let s1, x = green_eject s1 in
-    Some (yellow p1 child s1 chain, x)
-  | Chain (Y, Packet (p1, child, s1), chain) ->
+    Some (make_yellow p1 child s1 c, x)
+  | Chain (Y, Packet (p1, child, s1), c) ->
     let s1, x = yellow_eject s1 in
-    Some (red p1 child s1 chain, x)
+    Some (make_red p1 child s1 c, x)
