Sdeque/corev2.v
@@ -1,7 +1,7 @@
-From Coq Require Import ssreflect.
-From Coq Require Import Program List Arith Lia.
+From Coq Require Import Program List.
 Import ListNotations.
 From Equations Require Import Equations.
+Require Import Coq.Program.Equality.
 From Hammer Require Import Tactics.
 From AAC_tactics Require Import AAC.
 From AAC_tactics Require Import Instances.
@@ -10,656 +10,291 @@ Import Instances.Lists.
 From Color Require Import color.
 Import GYR.
 
-(* Types *)
+(* +------------------------------------------------------------------------+ *)
+(* |                                 Types                                  | *)
+(* +------------------------------------------------------------------------+ *)
 
-(* A type for iterated products. *)
-
+(* A type for leveled products. *)
 Inductive prodN (A : Type) : nat -> Type :=
   | prodZ : A -> prodN A 0
   | prodS {n : nat} : prodN A n -> prodN A n -> prodN A (S n).
 Arguments prodZ {A} a.
 Arguments prodS {A n} p1 p2.
 
-(* In the following types, an integer parameter is introduced : the [size] of
-   the type. The size is simply the number of [prodN A lvl] that are stored in
-   the structure encoded. *)
+(* A type for leveled options. *)
+Definition optionN (A : Type) (lvl : nat) := option (prodN A lvl).
 
-(* A type for sized buffers. *)
-
-Inductive buffer (A : Type) (lvl : nat) : nat -> color -> Type :=
-  | B0 : buffer A lvl 0 red
-  | B1 : prodN A lvl -> buffer A lvl 1 yellow
-  | B2 : prodN A lvl -> prodN A lvl -> buffer A lvl 2 green
-  | B3 : prodN A lvl -> prodN A lvl -> prodN A lvl -> buffer A lvl 3 green
-  | B4 : prodN A lvl -> prodN A lvl ->
-         prodN A lvl -> prodN A lvl -> buffer A lvl 4 yellow
-  | B5 : prodN A lvl -> prodN A lvl -> prodN A lvl ->
-         prodN A lvl -> prodN A lvl -> buffer A lvl 5 red.
+(* A type for buffers. *)
+Inductive buffer (A : Type) (lvl : nat) : color -> Type :=
+  | B0         : buffer A lvl red
+  | B1 {y r}   : prodN A lvl -> buffer A lvl (Mix NoGreen y r)
+  | B2 {g y r} : prodN A lvl -> prodN A lvl -> buffer A lvl (Mix g y r)
+  | B3 {g y r} : prodN A lvl -> prodN A lvl -> prodN A lvl ->
+                 buffer A lvl (Mix g y r)
+  | B4 {y r}   : prodN A lvl -> prodN A lvl -> prodN A lvl ->
+                 prodN A lvl -> buffer A lvl (Mix NoGreen y r)
+  | B5         : prodN A lvl -> prodN A lvl -> prodN A lvl ->
+                 prodN A lvl -> prodN A lvl -> buffer A lvl red.
 Arguments B0 {A lvl}.
-Arguments B1 {A lvl} a.
-Arguments B2 {A lvl} a b.
-Arguments B3 {A lvl} a b c.
-Arguments B4 {A lvl} a b c d.
-Arguments B5 {A lvl} a b c d e.
+Arguments B1 {A lvl y r}.
+Arguments B2 {A lvl g y r}.
+Arguments B3 {A lvl g y r}.
+Arguments B4 {A lvl y r}.
+Arguments B5 {A lvl}.
 
-(* A type for yellow buffers. *)
-
-Inductive yellow_buffer (A: Type) (lvl : nat) (size : nat) : Type :=
-  | Yellowish {G Y} :
-    buffer A lvl size (Mix G Y NoRed) -> yellow_buffer A lvl size.
-Arguments Yellowish {A lvl size G Y} b.
-
-(* A type for any buffers. *)
-
-Inductive any_buffer (A: Type) (lvl : nat) (size : nat) : Type :=
-  | Any {G Y R} :
-    buffer A lvl size (Mix G Y R) -> any_buffer A lvl size.
-Arguments Any {A lvl size G Y R} b.
-
-(* A relation between the prefix, suffix and packet colors. *)
-
-Inductive packet_color : color -> color -> color -> Type :=
-  | PCGreen : packet_color green green green
-  | PCYellow {G1 Y1 G2 Y2} :
-    packet_color (Mix G1 Y1 NoRed) (Mix G2 Y2 NoRed) yellow
-  | PCRed {G1 Y1 R1 G2 Y2 R2} :
-    packet_color (Mix G1 Y1 R1) (Mix G2 Y2 R2) red.
-
-(* A type for packet. As the level of the child packet is increased by one,
-   it contains elements of type [prodN A (S lvl)] that account for two elements
-   of type [prodN A lvl]. Hence, the size of the child packet is counted twice
-   in the size of our final packet of level [lvl]. *)
-
-Inductive packet (A : Type) (lvl : nat) : nat -> nat -> color -> Type :=
-  | Hole : packet A lvl lvl 0 uncolored
-  | Triple {tlvl psize pktsize ssize : nat} {Y} {C1 C2 C3 : color} :
-      buffer A lvl psize C1 ->
-      packet A (S lvl) tlvl pktsize (Mix NoGreen Y NoRed) ->
-      buffer A lvl ssize C2 ->
-      packet_color C1 C2 C3 ->
-      packet A lvl tlvl (psize + pktsize + pktsize + ssize) C3.
+(* A type for packets. *)
+Inductive packet (A : Type) (lvl : nat) : nat -> color -> Type :=
+  | Hole : packet A lvl lvl uncolored
+  | Packet {hlvl C y} : buffer A lvl C ->
+                        packet A (S lvl) hlvl (Mix NoGreen y NoRed) ->
+                        buffer A lvl C ->
+                        packet A lvl hlvl C.
 Arguments Hole {A lvl}.
-Arguments Triple {A lvl tlvl psize pktsize ssize Y C1 C2 C3} p pkt s pc.
+Arguments Packet {A lvl hlvl C y}.
 
-(* [power2] computes 2 to the power of a natural number. *)
+(* A type for the regularity relation. *)
+Inductive regularity : color -> color -> Type :=
+  | G {g r} : regularity green  (Mix g NoYellow r)
+  | Y       : regularity yellow green
+  | R       : regularity red    green.
 
-Equations power2 : nat -> nat :=
-power2 0 := 1;
-power2 (S n) := let p := power2 n in p + p.
-Transparent power2.
+(* A type for chains. *)
+Inductive chain (A : Type) : nat -> color -> Type :=
+  | Ending {lvl} : buffer A lvl red -> chain A lvl green
+  | Chain {lvl hlvl C1 C2} :
+      regularity C1 C2 -> packet A lvl hlvl C1 -> chain A hlvl C2 ->
+      chain A lvl C1.
+Arguments Ending {A lvl}.
+Arguments Chain {A lvl hlvl C1 C2}.
 
-(* A relation between the head packet and the following deque colors. *)
-
-Inductive cdeque_color : color -> color -> Type :=
-  | CCGreen {G R} : cdeque_color green (Mix G NoYellow R)
-  | CCYellow : cdeque_color yellow green
-  | CCRed : cdeque_color red green.
-
-(* A type for sized colored deque. The same reasonning as the one for packets
-   apply here. Each elements of the next colored deque accounts for [power2
-   len] elements of type [prodN A lvl]. So the size of the next colored deque
-   is multiplied by [power2 len] to compute the correct size for our colored
-   deque. *)
-
-Inductive cdeque (A : Type) (lvl : nat) : nat -> color -> Type :=
-  | Small {size : nat} {C : color} :
-      buffer A lvl size C ->
-      cdeque A lvl size green
-  | Big {tlvl pktsize nsize size : nat} {C1 C2 : color} :
-      packet A lvl tlvl pktsize C1 ->
-      cdeque A tlvl nsize C2 ->
-      size = pktsize + (power2 (tlvl - lvl)) * nsize ->
-      cdeque_color C1 C2 ->
-      cdeque A lvl size C1.
-Arguments Small {A lvl size C} b.
-Arguments Big {A lvl tlvl pktsize nsize size C1 C2} pkt cd eqsize cc.
-
-(* This function compute the size of an option. 0 if it is [None], 1 if it is
-   [Some _]. *)
-
-Equations size_option {A : Type} (o : option A) : nat :=
-size_option None := 0;
-size_option (Some _) := 1.
-Transparent size_option.
-
-(* The sized decompose type. *)
-
-Inductive decompose (A : Type) (lvl : nat) : nat -> Type :=
-  | Underflow (opt : option (prodN A lvl)) : decompose A lvl (size_option opt)
-  | Ok {size : nat} : buffer A lvl size green -> decompose A lvl size
-  | Overflow {size : nat} :
-    buffer A lvl size green -> prodN A (S lvl) -> decompose A lvl (2 + size).
+(* A type decomposing buffers according to their number of elements.
+   Buffers with 0 or 1 element are decomposed into [Underflow];
+   buffers with 2 or 3 elements are decomposed into [Ok];
+   buffers with 4 or 5 elements are decomposed into [Overflow]. *)
+Inductive decompose (A : Type) (lvl : nat) : Type :=
+  | Underflow : optionN A lvl -> decompose A lvl
+  | Ok : buffer A lvl green -> decompose A lvl
+  | Overflow : buffer A lvl green -> prodN A (S lvl) -> decompose A lvl.
 Arguments Underflow {A lvl}.
-Arguments Ok {A lvl size} b.
-Arguments Overflow {A lvl size} b ab.
+Arguments Ok {A lvl}.
+Arguments Overflow {A lvl}.
 
-(* The sized sandwich type. *)
-
-Inductive sandwich (A : Type) (lvl : nat) : nat -> Type :=
-  | Alone (opt : option (prodN A lvl)) : sandwich A lvl (size_option opt)
-  | Sandwich {size : nat} {C : color} :
-    prodN A lvl -> buffer A lvl size C -> prodN A lvl ->
-    sandwich A lvl (2 + size).
+(* A type decomposing a buffer into its first element, a central buffer, and
+   its last element. If such a decomposition is not possible, an option
+   representing the buffer is returned with [Alone]. *)
+Inductive sandwich (A : Type) (lvl : nat) : Type :=
+  | Alone : optionN A lvl -> sandwich A lvl
+  | Sandwich : prodN A lvl -> buffer A lvl red -> prodN A lvl -> sandwich A lvl.
 Arguments Alone {A lvl}.
-Arguments Sandwich {A lvl size C} ab b cd.
+Arguments Sandwich {A lvl}.
 
-(* A type for sized deque. *)
+(* A type for deque. *)
+Inductive deque (A : Type) : Type :=
+  | T {g y} : chain A 0 (Mix g y NoRed) -> deque A.
+Arguments T {A g y}.
 
-Inductive deque (A : Type) (size : nat) : Type :=
-  | T {G : green_hue} {Y : yellow_hue} :
-    cdeque A 0 size (Mix G Y NoRed) ->
-    deque A size.
-Arguments T {A size G Y} cd.
+(* +------------------------------------------------------------------------+ *)
+(* |                                 Models                                 | *)
+(* +------------------------------------------------------------------------+ *)
 
-(* Models *)
-
+(* Model functions are transparent. *)
 Set Equations Transparent.
 
-(* The list application is made opaque. *)
-
+(* The [app] function and the singleton list are made opaque. *)
 Opaque app.
 Definition singleton {A : Type} (x : A) : list A := [x].
 Opaque singleton.
 
-(* A list of tactics to be used when trying to resolve obligations generated by
-   Equations. *)
+(* Returns the sequence associated a product. *)
+Equations prodN_seq {A n} : prodN A n -> list A :=
+prodN_seq (prodZ a) := [a];
+prodN_seq (prodS p1 p2) := prodN_seq p1 ++ prodN_seq p2.
 
-#[export] Hint Rewrite <-app_assoc : rlist.
-#[export] Hint Rewrite <-app_comm_cons : rlist.
-#[export] Hint Rewrite app_nil_r : rlist.
-#[export] Hint Rewrite map_app : rlist.
-#[export] Hint Rewrite concat_app : rlist.
+(* Returns the sequence associated to an option. *)
+Equations optionN_seq {A lvl} : optionN A lvl -> list A :=
+optionN_seq None := [];
+optionN_seq (Some x) := prodN_seq x.
 
-#[local] Obligation Tactic :=
-  try first [ done | cbn; hauto db:rlist ].
-
-(* Returns the sequence contained in a product. *)
-
-Equations prodN_seq {A} (n : nat) : prodN A n -> list A :=
-prodN_seq 0 (prodZ a) := [a];
-prodN_seq (S n) (prodS p1 p2) := prodN_seq n p1 ++ prodN_seq n p2.
-Arguments prodN_seq {A n}.
-
-(* Returns the sequence contained in an option. *)
-
-Equations option_seq {A lvl} : option (prodN A lvl) -> list A :=
-option_seq None := [];
-option_seq (Some x) := prodN_seq x.
-
-(* Returns the sequence contained in a buffer. *)
-
-Equations buffer_seq {A lvl size C} : buffer A lvl size C -> list A :=
+(* Returns the sequence associated to a buffer. *)
+Equations buffer_seq {A lvl C} : buffer A lvl C -> list A :=
 buffer_seq B0 := [];
 buffer_seq (B1 a) := prodN_seq a;
 buffer_seq (B2 a b) := prodN_seq a ++ prodN_seq b;
 buffer_seq (B3 a b c) := prodN_seq a ++ prodN_seq b ++ prodN_seq c;
-buffer_seq (B4 a b c d) := prodN_seq a ++ prodN_seq b ++ prodN_seq c ++ prodN_seq d;
-buffer_seq (B5 a b c d e) :=
-  prodN_seq a ++ prodN_seq b ++ prodN_seq c ++ prodN_seq d ++ prodN_seq e.
+buffer_seq (B4 a b c d) := prodN_seq a ++ prodN_seq b ++ prodN_seq c ++
+                           prodN_seq d;
+buffer_seq (B5 a b c d e) := prodN_seq a ++ prodN_seq b ++ prodN_seq c ++
+                             prodN_seq d ++ prodN_seq e.
 
-(* Returns the sequence contained in a yellow buffer. *)
+(* Returns the sequence associated to a packet, provided the sequence
+   associated to its hole. *)
+Equations packet_seq {A lvl hlvl C} : packet A lvl hlvl C -> list A -> list A :=
+packet_seq Hole l := l;
+packet_seq (Packet p pkt s) l :=
+  buffer_seq p ++ packet_seq pkt l ++ buffer_seq s.
 
-Equations yellow_buffer_seq {A lvl size} : yellow_buffer A lvl size -> list A :=
-yellow_buffer_seq (Yellowish buf) := buffer_seq buf.
+(* Returns the sequence associated to a chain. *)
+Equations chain_seq {A lvl C} : chain A lvl C -> list A :=
+chain_seq (Ending b) := buffer_seq b;
+chain_seq (Chain _ pkt c) := packet_seq pkt (chain_seq c).
 
-(* Returns the sequence contained in any buffer. *)
-
-Equations any_buffer_seq {A lvl size} : any_buffer A lvl size -> list A :=
-any_buffer_seq (Any buf) := buffer_seq buf.
-
-(* Returns the sequence of elements stored in prefix buffers along a
-   packet. *)
-
-Equations packet_left_seq {A lvl len size C} : packet A lvl len size C -> list A :=
-packet_left_seq Hole := [];
-packet_left_seq (Triple buf1 p _ _) :=
-  buffer_seq buf1 ++ packet_left_seq p.
-
-(* Returns the sequence of elements stored in suffix buffers along a
-   packet. *)
-
-Equations packet_right_seq {A lvl len size C} : packet A lvl len size C -> list A :=
-packet_right_seq Hole := [];
-packet_right_seq (Triple _ p buf2 _) :=
-  packet_right_seq p ++ buffer_seq buf2.
-
-(* Returns the sequence contained in a colored deque. *)
-
-Equations cdeque_seq {A lvl size C} : cdeque A lvl size C -> list A :=
-cdeque_seq (Small buf) := buffer_seq buf;
-cdeque_seq (Big p cd _ _) :=
-    packet_left_seq p ++
-    cdeque_seq cd ++
-    packet_right_seq p.
-
-(* Returns the sequence of non-excess elements of an object of type decompose. *)
-
-Equations decompose_main_seq {A lvl size} (dec : decompose A lvl size) : list A :=
-decompose_main_seq (Underflow opt) := option_seq opt;
+(* Returns the first 4 elements of the sequence associated to a decomposed
+   buffer.*)
+Equations decompose_main_seq {A lvl} (dec : decompose A lvl) : list A :=
+decompose_main_seq (Underflow opt) := optionN_seq opt;
 decompose_main_seq (Ok b) := buffer_seq b;
 decompose_main_seq (Overflow b _) := buffer_seq b.
 
-(* Returns the sequence of excess elements of an object of type decompose. *)
-
-Equations decompose_rest_seq {A lvl size} (dec : decompose A lvl size) : list A :=
+(* Returns the sequence associated to a decomposed buffer from the 5th element
+   to the end  *)
+Equations decompose_rest_seq {A lvl} (dec : decompose A lvl) : list A :=
 decompose_rest_seq (Underflow _) := [];
 decompose_rest_seq (Ok _) := [];
 decompose_rest_seq (Overflow _ p) := prodN_seq p.
 
-(* Returns the sequence of elements of an object of type sandwich. *)
-
-Equations sandwich_seq {A lvl size} (sw : sandwich A lvl size) : list A :=
-sandwich_seq (Alone opt) := option_seq opt;
+(* Returns the sequence associated to a sandwiched buffer. *)
+Equations sandwich_seq {A lvl} (sw : sandwich A lvl) : list A :=
+sandwich_seq (Alone opt) := optionN_seq opt;
 sandwich_seq (Sandwich x b y) := prodN_seq x ++ buffer_seq b ++ prodN_seq y.
 
-(* Returns the sequence contained in a deque. *)
-
-Equations deque_seq {A size} : deque A size -> list A :=
-deque_seq (T dq) := cdeque_seq dq.
+(* Returns the sequence associated to a deque. *)
+Equations deque_seq {A} : deque A -> list A :=
+deque_seq (T dq) := chain_seq dq.
 
 Unset Equations Transparent.
 
-(* Sequence mappings *)
+(* +------------------------------------------------------------------------+ *)
+(* |                                  Core                                  | *)
+(* +------------------------------------------------------------------------+ *)
 
-Definition map_deque {T : Type -> nat -> Type} {A : Type}
-  (f : forall {lvl : nat}, T A lvl -> list A)
-  {lvl q : nat}
-  (d : deque (T A lvl) q) : list A :=
-  let fix prodN_seq {lvlt lvlp} (p : prodN (T A lvlt) lvlp) {struct p} : list A :=
-    match p with
-    | prodZ z => f z
-    | prodS p1 p2 => prodN_seq p1 ++ prodN_seq p2
-    end in
-  let buffer_seq {lvlt lvlp size C} (b : buffer (T A lvlt) lvlp size C) : list A :=
-    match b with
-    | B0 => []
-    | B1 p1 => prodN_seq p1
-    | B2 p1 p2 => prodN_seq p1 ++ prodN_seq p2
-    | B3 p1 p2 p3 => prodN_seq p1 ++ prodN_seq p2 ++ prodN_seq p3
-    | B4 p1 p2 p3 p4 =>
-      prodN_seq p1 ++ prodN_seq p2 ++ prodN_seq p3 ++ prodN_seq p4
-    | B5 p1 p2 p3 p4 p5 =>
-      prodN_seq p1 ++ prodN_seq p2 ++ prodN_seq p3 ++ prodN_seq p4 ++ prodN_seq p5
-    end in
-  let fix packet_left_seq {lvlt lvlp len size C}
-      (pkt : packet (T A lvlt) lvlp len size C) {struct pkt} : list A :=
-    match pkt with
-    | Hole => []
-    | Triple p pkt _ _ => buffer_seq p ++ packet_left_seq pkt
-    end in
-  let fix packet_right_seq {lvlt lvlp len size C}
-      (pkt : packet (T A lvlt) lvlp len size C) {struct pkt} : list A :=
-    match pkt with
-    | Hole => []
-    | Triple _ pkt s _ => packet_right_seq pkt ++ buffer_seq s
-    end in
-  let fix cdeque_seq {lvlt lvlp size C}
-      (cd : cdeque (T A lvlt) lvlp size C) {struct cd} : list A :=
-    match cd with
-    | Small b => buffer_seq b
-    | Big pkt cd _ _ =>
-      packet_left_seq pkt ++
-      cdeque_seq cd ++
-      packet_right_seq pkt
-    end in
-  match d with
-  | T cd => cdeque_seq cd
-  end.
-
-(* A lemma that destructs an equality of one app into 2 subgoals. *)
-
-Lemma div_app2 {A : Type} {l1 l1' l2 l2' : list A} :
-    l1 = l1' -> l2 = l2' -> l1 ++ l2 = l1' ++ l2'.
-Proof. intros [] []; reflexivity. Qed.
-
-(* A tactic that cleans the removes the useless hypothesis. *)
-
-Local Ltac clear_h :=
-  repeat
-  match goal with
-  | H : _ |- _ => clear H
-  end.
-
-Lemma correct_mapping {T : Type -> nat -> Type} {A : Type}
-  (f : forall {lvl : nat}, T A lvl -> list A)
-  {lvl q : nat}
-  (d : deque (T A lvl) q) :
-  map_deque (@f) d = concat (map f (deque_seq d)).
-Proof.
-  (* Destruction of the deque. *)
-  destruct d as [G Y cd]; cbn;
-  (* Induction on the cdeque. *)
-  induction cd as [lvlp size C b | lvlp len pktsize nsize size C1 C2 pkt cd IHcd esize cc];
-  (* Format for simplification. *)
-  cbn; autorewrite with rlist;
-  (* Handling the Big case, with packets and a following cdeque. *)
-  try (repeat apply div_app2;
-  (* The following cdeque case is handled by induction. *)
-  [clear_h | apply IHcd | clear_h];
-  (* Induction on the packet. *)
-  induction pkt as [ | lvlp ???????? p pkt IHpkt s pc];
-  (* Hole cases. *)
-  try reflexivity;
-  (* Format for simplification. *)
-  cbn; autorewrite with rlist;
-  (* Separate buffer and following packet cases. *)
-  apply div_app2;
-  (* Following packet cases are handled by induction. *)
-  [clear_h; rename p into b | apply IHpkt | apply IHpkt | clear_h; rename s into b]);
-  (* Case by case on buffers. *)
-  destruct b;
-  (* Format for simplification. *)
-  cbn; autorewrite with rlist;
-  (* Simple B0 cases are handled. *)
-  try reflexivity;
-  (* Separate multi-app goals into subgoals. *)
-  repeat apply div_app2; clear_h;
-  (* Prove the remaining by induction on the right prodN. *)
-  (match goal with
-  | _ : _ |- _ = concat (map (f lvl) (prodN_seq ?p)) => induction p
-  end);
-  (* Finish all the cases with hauto. *)
-  cbn; hauto db:rlist.
-Qed.
-
+(* Notation for dependent types hiding the property on [x]. *)
 Notation "? x" := (@exist _ _ x _) (at level 100).
 
-(* Lemmas *)
+(* A hint database of rewrites to be used when trying to automatically resolve
+   obligations generated by [Equations]. *)
+#[export] Hint Rewrite <-app_assoc : rlist.
+#[export] Hint Rewrite app_nil_r : rlist.
 
-(* Proves that for any natural number [n], [power2 n] is different from 0. *)
-
-Lemma power2_neq0 {n : nat} : power2 n <> 0.
-Proof. induction n; simpl; lia. Qed.
-
-(* Takes a product and links its level to the length of its sequence. *)
-
-Lemma prodN_size {A lvl} (p : prodN A lvl) :
-    length (prodN_seq p) = power2 lvl.
-Proof.
-  induction p.
-  - reflexivity.
-  - simp prodN_seq; simpl power2;
-    rewrite app_length;
-    rewrite IHp1; rewrite IHp2;
-    reflexivity.
-Qed.
-
-(* Takes an option of products and links its level and size to the length of its
-   sequence. *)
-
-Lemma option_size {A lvl} (o : option (prodN A lvl)) :
-    length (option_seq o) = size_option o * power2 lvl.
-Proof.
-  destruct o; simp option_seq; try reflexivity;
-  simp size_option; rewrite Nat.mul_1_l; apply prodN_size.
-Qed.
-
-(* Takes a buffer and links its level and size to the length of its sequence. *)
-
-Lemma buffer_size {A lvl size C} (b : buffer A lvl size C) :
-    length (buffer_seq b) = size * power2 lvl.
-Proof.
-  dependent destruction b;
-  simp buffer_seq;
-  repeat rewrite app_length;
-  repeat rewrite prodN_size;
-  cbn; lia.
-Qed.
-
-(* Proves that if a buffer is empty, its size is 0. *)
-
-Lemma empty_buffer_size {A lvl size C} (b : buffer A lvl size C) :
-    buffer_seq b = [] -> size = 0.
-Proof.
-  intros e%(f_equal (@length _)); rewrite buffer_size in e;
-  apply Nat.mul_eq_0_l in e.
-  - assumption.
-  - apply power2_neq0.
-Qed.
-
-(* Takes a packet and links its level and size to the length of its sequence. *)
-
-Lemma packet_size {A lvl len size C} (pkt : packet A lvl len size C) :
-    length (packet_left_seq pkt ++ packet_right_seq pkt) = size * power2 lvl.
-Proof.
-  induction pkt.
-  - reflexivity.
-  - simp packet_left_seq packet_right_seq;
-    autorewrite with rlist;
-    rewrite app_length;
-    rewrite app_assoc; rewrite app_length;
-    repeat rewrite buffer_size;
-    do 2 rewrite Nat.mul_add_distr_r;
-    rewrite IHpkt; cbn; lia.
-Qed.
-
-(* A simple lemma to better control list concatenation. *)
-
-Lemma app_cons {A : Type} (a : A) (l : list A) :
-    a :: l = [a] ++ l.
-Proof. reflexivity. Qed.
-
-(* Proves the commutation of list under the length function. *)
-
-Lemma length_app_comm {A : Type} (l1 l2 : list A) :
-    length (l1 ++ l2) = length (l2 ++ l1).
-Proof.
-  induction l1 as [ | a l1]; try rewrite app_cons;
-  repeat rewrite app_length; lia.
-Qed.
-
-(* Proves that 2 ^ (n + m) is indeed equal to 2 ^ n * 2 ^ m. *)
-
-Lemma power2_add {n m : nat} : power2 (n + m) = power2 n * power2 m.
-Proof.
-  induction n; simpl.
-  - lia.
-  - rewrite IHn Nat.mul_add_distr_r; reflexivity.
-Qed.
-
-(* Proves that 2 ^ (n - m) is equal to 2 ^ n / 2 ^ m if m <= n. *)
-
-Lemma power2_sub {n m : nat} : m <= n -> power2 (n - m) = power2 n / power2 m.
-Proof.
-  revert m. induction n; simpl.
-  - intros m I%(Nat.le_0_r). subst. reflexivity.
-  - intros m I.
-    destruct m.
-    + simpl power2. rewrite Nat.div_1_r. reflexivity.
-    + simpl power2. etransitivity.
-      -- apply IHn, le_S_n. exact I.
-      -- symmetry.
-         assert (forall p, p + p = 2 * p). { lia. }
-         do 2 rewrite H.
-         apply Nat.Div0.div_mul_cancel_l.
-         lia.
-Qed.
-
-Lemma packet_lvl_ineq {A lvl tlvl size C} (pkt : packet A lvl tlvl size C) :
-  lvl <= tlvl.
-Proof. induction pkt; lia. Qed.
-
-(* Takes a colored deque and links its level and size to the length of its
-   sequence. *)
-
-Lemma cdeque_size {A lvl size C} (cd : cdeque A lvl size C) :
-    length (cdeque_seq cd) = size * power2 lvl.
-Proof.
-  induction cd; simp cdeque_seq.
-  - apply buffer_size.
-  - rewrite app_assoc length_app_comm app_assoc app_length length_app_comm packet_size.
-    rewrite IHcd e.
-    rewrite power2_sub.
-    + eapply packet_lvl_ineq. exact p.
-    + admit.
-Qed.
-
-(* Takes a deque and links its size to the length of its sequence. *)
-
-Lemma deque_size {A size} (d : deque A size) : length (deque_seq d) = size.
-Proof. destruct d; simp deque_seq; rewrite cdeque_size; simpl; lia. Qed.
-
-(* Elements *)
-
-(* The empty colored deque. *)
-
-Equations cempty {A lvl} : { cd : cdeque A lvl 0 green | cdeque_seq cd = [] } :=
-cempty := ? Small B0.
-
-(* The empty deque. *)
-
-Equations empty {A} : { d : deque A 0 | deque_seq d = [] } :=
-empty with cempty => { | ? cd := ? T cd }.
-
-(* Functions *)
-
+(* Setting the default tactics for obligations to be [hauto] using the [rlist]
+   hint database. *)
 #[local] Obligation Tactic :=
-  try first [ done | cbn; hauto db:rlist ].
+  try first [ cbn; hauto db:rlist ].
 
-(* Pushing on a green buffer. *)
-
-Equations green_push {A lvl size}
-  (x : prodN A lvl) (b : buffer A lvl size green) :
-  { b' : buffer A lvl (S size) yellow |
-    buffer_seq b' = prodN_seq x ++ buffer_seq b } :=
-green_push x (B2 a b) := ? B3 x a b;
+(* Pushes on a green buffer. *)
+Equations green_push {A lvl} (x : prodN A lvl) (b : buffer A lvl green) :
+  { b' : buffer A lvl yellow | buffer_seq b' = prodN_seq x ++ buffer_seq b } :=
+green_push x (B2 a b)   := ? B3 x a b;
 green_push x (B3 a b c) := ? B4 x a b c.
 
-(* Injecting on a green buffer. *)
-
-Equations green_inject {A lvl size}
-  (b : buffer A lvl size green) (x : prodN A lvl) :
-  { b' : buffer A lvl (S size) yellow |
-    buffer_seq b' = buffer_seq b ++ prodN_seq x } :=
-green_inject (B2 a b) x := ? B3 a b x;
+(* Injects on a green buffer. *)
+Equations green_inject {A lvl} (b : buffer A lvl green) (x : prodN A lvl) :
+  { b' : buffer A lvl yellow | buffer_seq b' = buffer_seq b ++ prodN_seq x } :=
+green_inject (B2 a b)   x := ? B3 a b x;
 green_inject (B3 a b c) x := ? B4 a b c x.
 
-(* Poping from a green buffer. *)
+(* Pops off a green buffer. *)
+Equations green_pop {A lvl} (b : buffer A lvl green) :
+  { '(x, b') : prodN A lvl * buffer A lvl yellow |
+    buffer_seq b = prodN_seq x ++ buffer_seq b' } :=
+green_pop (B2 a b)   => ? (a, B1 b);
+green_pop (B3 a b c) => ? (a, B2 b c).
 
-Equations green_pop {A lvl size} (b : buffer A lvl size green) :
-  { '(x, b') : prodN A lvl * yellow_buffer A lvl (Nat.pred size) |
-    buffer_seq b = prodN_seq x ++ yellow_buffer_seq b' } :=
-green_pop (B2 a b) => ? (a, (Yellowish (B1 b)));
-green_pop (B3 a b c) => ? (a, (Yellowish (B2 b c))).
+(* Ejects off a green buffer. *)
+Equations green_eject {A lvl} (b : buffer A lvl green) :
+  { '(b', x) : buffer A lvl yellow * prodN A lvl |
+    buffer_seq b = buffer_seq b' ++ prodN_seq x } :=
+green_eject (B2 a b)   => ? (B1 a, b);
+green_eject (B3 a b c) => ? (B2 a b, c).
 
-(* Ejecting from a green buffer. *)
+(* Pushes on a yellow buffer. *)
+Equations yellow_push {A lvl} (x : prodN A lvl) (b : buffer A lvl yellow) :
+  { b' : buffer A lvl red | buffer_seq b' = prodN_seq x ++ buffer_seq b } :=
+yellow_push x (B1 a)       := ? B2 x a;
+yellow_push x (B2 a b)     := ? B3 x a b;
+yellow_push x (B3 a b c)   := ? B4 x a b c;
+yellow_push x (B4 a b c d) := ? B5 x a b c d.
 
-Equations green_eject {A lvl size} (b : buffer A lvl size green) :
-  { '(b', x) : yellow_buffer A lvl (Nat.pred size) * prodN A lvl |
-    buffer_seq b = yellow_buffer_seq b' ++ prodN_seq x } :=
-green_eject (B2 a b) => ? ((Yellowish (B1 a)), b);
-green_eject (B3 a b c) => ? ((Yellowish (B2 a b)), c).
+(* Injects on a yellow buffer. *)
+Equations yellow_inject {A lvl} (b : buffer A lvl yellow) (x : prodN A lvl) :
+  { b' : buffer A lvl red | buffer_seq b' = buffer_seq b ++ prodN_seq x } :=
+yellow_inject (B1 a)       x := ? B2 a x;
+yellow_inject (B2 a b)     x := ? B3 a b x;
+yellow_inject (B3 a b c)   x := ? B4 a b c x;
+yellow_inject (B4 a b c d) x := ? B5 a b c d x.
 
-(* Pushing on a yellow buffer. *)
+(* Pops off a yellow buffer. *)
+Equations yellow_pop {A lvl} (b : buffer A lvl yellow) :
+  { '(x, b') : prodN A lvl * buffer A lvl red |
+    buffer_seq b = prodN_seq x ++ buffer_seq b' } :=
+yellow_pop (B1 a)       := ? (a, B0);
+yellow_pop (B2 a b)     := ? (a, B1 b);
+yellow_pop (B3 a b c)   := ? (a, B2 b c);
+yellow_pop (B4 a b c d) := ? (a, B3 b c d).
 
-#[derive(eliminator=no)]
-Equations yellow_push {A lvl size}
-  (x : prodN A lvl) (b : yellow_buffer A lvl size) :
-  { b' : any_buffer A lvl (S size) |
-    any_buffer_seq b' = prodN_seq x ++ yellow_buffer_seq b } :=
-yellow_push x (Yellowish buf) with buf => {
-  | B1 a => ? Any (B2 x a);
-  | B2 a b => ? Any (B3 x a b);
-  | B3 a b c => ? Any (B4 x a b c);
-  | B4 a b c d => ? Any (B5 x a b c d)
-}.
+(* Ejects off a yellow buffer. *)
+Equations yellow_eject {A lvl} (b : buffer A lvl yellow) :
+  { '(b', x) : buffer A lvl red * prodN A lvl |
+    buffer_seq b = buffer_seq b' ++ prodN_seq x } :=
+yellow_eject (B1 a)       := ? (B0, a);
+yellow_eject (B2 a b)     := ? (B1 a, b);
+yellow_eject (B3 a b c)   := ? (B2 a b, c);
+yellow_eject (B4 a b c d) := ? (B3 a b c, d).
 
-(* Injecting on a yellow buffer. *)
-
-#[derive(eliminator=no)]
-Equations yellow_inject {A lvl size}
-  (b : yellow_buffer A lvl size) (x : prodN A lvl) :
-  { b' : any_buffer A lvl (S size) |
-    any_buffer_seq b' = yellow_buffer_seq b ++ prodN_seq x } :=
-yellow_inject (Yellowish buf) x with buf := {
-  | B1 a => ? Any (B2 a x);
-  | B2 a b => ? Any (B3 a b x);
-  | B3 a b c => ? Any (B4 a b c x);
-  | B4 a b c d => ? Any (B5 a b c d x)
-}.
-
-(* Poping from a yellow buffer. *)
-
-#[derive(eliminator=no)]
-Equations yellow_pop {A lvl size} (b : yellow_buffer A lvl size) :
-  { '(x, b') : prodN A lvl * any_buffer A lvl (Nat.pred size) |
-    yellow_buffer_seq b = prodN_seq x ++ any_buffer_seq b' } :=
-yellow_pop (Yellowish buf) with buf => {
-  | B1 a => ? (a, Any B0);
-  | B2 a b => ? (a, Any (B1 b));
-  | B3 a b c => ? (a, Any (B2 b c));
-  | B4 a b c d => ? (a, Any (B3 b c d))
-}.
-
-(* Ejecting from a yellow buffer. *)
-
-#[derive(eliminator=no)]
-Equations yellow_eject {A lvl size} (b : yellow_buffer A lvl size) :
-  { '(b', x) : any_buffer A lvl (Nat.pred size) * prodN A lvl |
-    yellow_buffer_seq b = any_buffer_seq b' ++ prodN_seq x } :=
-yellow_eject (Yellowish buf) with buf => {
-  | B1 a => ? (Any B0, a);
-  | B2 a b => ? (Any (B1 a), b);
-  | B3 a b c => ? (Any (B2 a b), c);
-  | B4 a b c d => ? (Any (B3 a b c), d)
-}.
-
-(* Pushing on a buffer. *)
-
-Equations buffer_push {A lvl size C} (x : prodN A lvl) (b : buffer A lvl size C) :
-  { cd : cdeque A lvl (S size) green |
-    cdeque_seq cd = prodN_seq x ++ buffer_seq b } :=
-buffer_push x B0 := ? Small (B1 x);
-buffer_push x (B1 a) := ? Small (B2 x a);
-buffer_push x (B2 a b) := ? Small (B3 x a b);
-buffer_push x (B3 a b c) := ? Small (B4 x a b c);
-buffer_push x (B4 a b c d) := ? Small (B5 x a b c d);
+(* Pushes on a buffer, and returns a green chain. *)
+Equations buffer_push {A lvl C} (x : prodN A lvl) (b : buffer A lvl C) :
+  { cd : chain A lvl green | chain_seq cd = prodN_seq x ++ buffer_seq b } :=
+buffer_push x B0 := ? Ending (B1 x);
+buffer_push x (B1 a) := ? Ending (B2 x a);
+buffer_push x (B2 a b) := ? Ending (B3 x a b);
+buffer_push x (B3 a b c) := ? Ending (B4 x a b c);
+buffer_push x (B4 a b c d) := ? Ending (B5 x a b c d);
 buffer_push x (B5 a b c d e) :=
-  ? Big (Triple (B3 x a b) Hole (B3 c d e) PCGreen) (Small B0) eq_refl _ CCGreen.
+    ? Chain G (Packet (B3 x a b) Hole (B3 c d e)) (Ending B0).
 
-(* Injecting on a buffer. *)
-
-Equations buffer_inject {A lvl size C} (b : buffer A lvl size C) (x : prodN A lvl) :
-  { cd : cdeque A lvl (S size) green |
-    cdeque_seq cd = buffer_seq b ++ prodN_seq x } :=
-buffer_inject B0 x := ? Small (B1 x);
-buffer_inject (B1 a) x := ? Small (B2 a x);
-buffer_inject (B2 a b) x := ? Small (B3 a b x);
-buffer_inject (B3 a b c) x := ? Small (B4 a b c x);
-buffer_inject (B4 a b c d) x := ? Small (B5 a b c d x);
+(* Injects on a buffer, and returns a green chain. *)
+Equations buffer_inject {A lvl C} (b : buffer A lvl C) (x : prodN A lvl) :
+  { cd : chain A lvl green | chain_seq cd = buffer_seq b ++ prodN_seq x } :=
+buffer_inject B0 x := ? Ending (B1 x);
+buffer_inject (B1 a) x := ? Ending (B2 a x);
+buffer_inject (B2 a b) x := ? Ending (B3 a b x);
+buffer_inject (B3 a b c) x := ? Ending (B4 a b c x);
+buffer_inject (B4 a b c d) x := ? Ending (B5 a b c d x);
 buffer_inject (B5 a b c d e) x :=
-  ? Big (Triple (B3 a b c) Hole (B3 d e x) PCGreen) (Small B0) eq_refl _ CCGreen.
+    ? Chain G (Packet (B3 a b c) Hole (B3 d e x)) (Ending B0).
 
-(* Poping from a buffer. *)
-
-Equations buffer_pop {A lvl size C} (b : buffer A lvl size C) :
-  { o : option (prodN A lvl * any_buffer A lvl (Nat.pred size)) |
+(* Pops off a buffer, and returns an option. *)
+Equations buffer_pop {A lvl C} (b : buffer A lvl C) :
+  { o : option (prodN A lvl * buffer A lvl red) |
     buffer_seq b =
     match o with
     | None => []
-    | Some (x, b') => prodN_seq x ++ any_buffer_seq b'
+    | Some (x, b') => prodN_seq x ++ buffer_seq b'
     end } :=
 buffer_pop B0 := ? None;
-buffer_pop (B5 a b c d e) := ? Some (a, Any (B4 b c d e));
-buffer_pop buf with yellow_pop (Yellowish buf) => { | ? o := ? Some o }.
+buffer_pop (B1 a) := ? Some (a, B0);
+buffer_pop (B2 a b) := ? Some (a, B1 b);
+buffer_pop (B3 a b c) := ? Some (a, B2 b c);
+buffer_pop (B4 a b c d) := ? Some (a, B3 b c d);
+buffer_pop (B5 a b c d e) := ? Some (a, B4 b c d e).
 
-(* Ejecting from a buffer. *)
-
-Equations buffer_eject {A lvl size C} (b : buffer A lvl size C) :
-  { o : option (any_buffer A lvl (Nat.pred size) * prodN A lvl) |
+(* Ejects off a buffer, and returns an option. *)
+Equations buffer_eject {A lvl C} (b : buffer A lvl C) :
+  { o : option (buffer A lvl red * prodN A lvl) |
     buffer_seq b =
     match o with
     | None => []
-    | Some (b', x) => any_buffer_seq b' ++ prodN_seq x
+    | Some (b', x) => buffer_seq b' ++ prodN_seq x
     end } :=
-buffer_eject (B5 a b c d e) := ? Some (Any (B4 a b c d), e);
 buffer_eject B0 := ? None;
-buffer_eject buf with yellow_eject (Yellowish buf) => { | ? o := ? Some o }.
+buffer_eject (B1 a) := ? Some (B0, a);
+buffer_eject (B2 a b) := ? Some (B1 a, b);
+buffer_eject (B3 a b c) := ? Some (B2 a b, c);
+buffer_eject (B4 a b c d) := ? Some (B3 a b c, d);
+buffer_eject (B5 a b c d e) := ? Some (B4 a b c d, e).
 
 (* Pushes then ejects. *)
-
-Equations prefix_rot {A lvl size C} (x : prodN A lvl) (b : buffer A lvl size C) :
-  { '(b', y) : buffer A lvl size C * prodN A lvl |
+Equations prefix_rot {A lvl C} (x : prodN A lvl) (b : buffer A lvl C) :
+  { '(b', y) : buffer A lvl C * prodN A lvl |
     prodN_seq x ++ buffer_seq b = buffer_seq b' ++ prodN_seq y } :=
 prefix_rot x B0 := ? (B0, x);
 prefix_rot x (B1 a) := ? (B1 x, a);
@@ -669,9 +304,8 @@ prefix_rot x (B4 a b c d) := ? (B4 x a b c, d);
 prefix_rot x (B5 a b c d e) := ? (B5 x a b c d, e).
 
 (* Injects then pops. *)
-
-Equations suffix_rot {A lvl size C} (b : buffer A lvl size C) (y : prodN A lvl) :
-  { '(x, b') : prodN A lvl * buffer A lvl size C |
+Equations suffix_rot {A lvl C} (b : buffer A lvl C) (y : prodN A lvl) :
+  { '(x, b') : prodN A lvl * buffer A lvl C |
     buffer_seq b ++ prodN_seq y = prodN_seq x ++ buffer_seq b' } :=
 suffix_rot B0 x := ? (x, B0);
 suffix_rot (B1 a) x := ? (a, B1 x);
@@ -680,62 +314,51 @@ suffix_rot (B3 a b c) x := ? (a, B3 b c x);
 suffix_rot (B4 a b c d) x := ? (a, B4 b c d x);
 suffix_rot (B5 a b c d e) x := ? (a, B5 b c d e x).
 
-(* Create a green buffer by injecting a pair onto an option. *)
-
-Equations prefix23 {A lvl G Y} (o : option (prodN A lvl)) (p: prodN A (S lvl)) :
-  { b : buffer A lvl (2 + size_option o) (Mix G Y NoRed) |
-    buffer_seq b = option_seq o ++ prodN_seq p } :=
-prefix23 None (prodS b c) := ? B2 b c;
+(* Merges an option and a pair to create a green buffer. *)
+Equations prefix23 {A lvl} (o : optionN A lvl) (p: prodN A (S lvl)) :
+  { b : buffer A lvl green | buffer_seq b = optionN_seq o ++ prodN_seq p } :=
+prefix23  None    (prodS b c) := ? B2 b c;
 prefix23 (Some a) (prodS b c) := ? B3 a b c.
 
-(* Create a green buffer by poping a pair onto an option. *)
-
-Equations suffix23 {A lvl G Y} (p : prodN A (S lvl)) (o : option (prodN A lvl)) :
-  { b : buffer A lvl (2 + size_option o) (Mix G Y NoRed) |
-    buffer_seq b = prodN_seq p ++ option_seq o } :=
-suffix23 (prodS a b) None := ? B2 a b;
+(* Merges a pair and an option to create a green buffer. *)
+Equations suffix23 {A lvl} (p : prodN A (S lvl)) (o : optionN A lvl) :
+  { b : buffer A lvl green | buffer_seq b = prodN_seq p ++ optionN_seq o } :=
+suffix23 (prodS a b)  None    := ? B2 a b;
 suffix23 (prodS a b) (Some c) := ? B3 a b c.
 
-(* Create a yellow (or green) buffer by pushing an element onto an option. *)
-
-Equations suffix12 {A lvl} (x : prodN A lvl) (o : option (prodN A lvl)) :
-  { b : buffer A lvl (S (size_option o)) yellow |
-    buffer_seq b = prodN_seq x ++ option_seq o } :=
-suffix12 x None := ? B1 x;
-suffix12 x (Some y) := ? B2 x y.
+(* Merges an element and an option to create a yellow buffer. *)
+Equations prefix12 {A lvl} (x : prodN A lvl) (o : optionN A lvl) :
+  { b : buffer A lvl yellow | buffer_seq b = prodN_seq x ++ optionN_seq o } :=
+prefix12 x  None    := ? B1 x;
+prefix12 x (Some y) := ? B2 x y.
 
 (* Returns the decomposed version of a buffer. Here, it is a prefix
-   decomposition: when the buffer is overflowed, elements at the end are
-   removed. *)
-
-Equations prefix_decompose {A lvl size C} (b : buffer A lvl size C) :
-  { dec : decompose A lvl size |
-    buffer_seq b = decompose_main_seq dec ++ decompose_rest_seq dec } :=
+   decomposition: when the buffer has 4 or 5 elements, those at the end are
+   set appart. *)
+Equations prefix_decompose {A lvl C} (b : buffer A lvl C) :
+  { dec : decompose A lvl | buffer_seq b = decompose_main_seq dec ++ decompose_rest_seq dec } :=
 prefix_decompose B0 := ? Underflow None;
-prefix_decompose (B1 x) := ? Underflow (Some x);
+prefix_decompose (B1 a) := ? Underflow (Some a);
 prefix_decompose (B2 a b) := ? Ok (B2 a b);
 prefix_decompose (B3 a b c) := ? Ok (B3 a b c);
 prefix_decompose (B4 a b c d) := ? Overflow (B2 a b) (prodS c d);
 prefix_decompose (B5 a b c d e) := ? Overflow (B3 a b c) (prodS d e).
 
 (* Returns the decomposed version of a buffer. Here, it is a suffix
-   decomposition: when the buffer is overflowed, elements at the beginning are
-   removed. *)
-
-Equations suffix_decompose {A lvl size C} (b : buffer A lvl size C) :
-  { dec : decompose A lvl size |
-    buffer_seq b = decompose_rest_seq dec ++ decompose_main_seq dec } :=
+   decomposition: when the buffer has 4 or 5 elements, those at the start are
+   set appart. *)
+Equations suffix_decompose {A lvl C} (b : buffer A lvl C) :
+  { dec : decompose A lvl | buffer_seq b = decompose_rest_seq dec ++ decompose_main_seq dec } :=
 suffix_decompose B0 := ? Underflow None;
-suffix_decompose (B1 x) := ? Underflow (Some x);
+suffix_decompose (B1 a) := ? Underflow (Some a);
 suffix_decompose (B2 a b) := ? Ok (B2 a b);
 suffix_decompose (B3 a b c) := ? Ok (B3 a b c);
 suffix_decompose (B4 a b c d) := ? Overflow (B2 c d) (prodS a b);
 suffix_decompose (B5 a b c d e) := ? Overflow (B3 c d e) (prodS a b).
 
-(* Returns the sandwich representation of a buffer. *)
-
-Equations buffer_unsandwich {A lvl size C} (b : buffer A lvl size C) :
-  { sw : sandwich A lvl size | buffer_seq b = sandwich_seq sw } :=
+(* Returns the sandwiched version of a buffer. *)
+Equations buffer_unsandwich {A lvl C} (b : buffer A lvl C) :
+  { sw : sandwich A lvl | buffer_seq b = sandwich_seq sw } :=
 buffer_unsandwich B0 := ? Alone None;
 buffer_unsandwich (B1 a) := ? Alone (Some a);
 buffer_unsandwich (B2 a b) := ? Sandwich a B0 b;
@@ -743,506 +366,309 @@ buffer_unsandwich (B3 a b c) := ? Sandwich a (B1 b) c;
 buffer_unsandwich (B4 a b c d) := ? Sandwich a (B2 b c) d;
 buffer_unsandwich (B5 a b c d e) := ? Sandwich a (B3 b c d) e.
 
-(* In the following, when talking about structures, we will write n-struct for
-   a structure of level n. *)
+(* In the following, n-buffer denote a buffer of level n. *)
 
-(* Translates a n-buffer to a (n+1)-buffer. An additional option type is
-   returned to handle cases where the buffer contains an odd number of elements. *)
+(* Converts a n-buffer to a (n+1)-buffer. If the buffer has an odd number of
+   elements, the first is returned via an option. *)
+Equations buffer_halve {A lvl C} (b : buffer A lvl C) :
+  { '(o, b') : optionN A lvl * buffer A (S lvl) red |
+    buffer_seq b = optionN_seq o ++ buffer_seq b' } :=
+buffer_halve B0 := ? (None, B0);
+buffer_halve (B1 a) := ? (Some a, B0);
+buffer_halve (B2 a b) := ? (None, B1 (prodS a b));
+buffer_halve (B3 a b c) := ? (Some a, B1 (prodS b c));
+buffer_halve (B4 a b c d) := ? (None, B2 (prodS a b) (prodS c d));
+buffer_halve (B5 a b c d e) := ? (Some a, B2 (prodS b c) (prodS d e)).
 
-Equations buffer_halve {A lvl size C} (b : buffer A lvl size C) :
-  { '(o, b') : option (prodN A lvl) * any_buffer A (S lvl) (size / 2) |
-    buffer_seq b = option_seq o ++ any_buffer_seq b' } :=
-buffer_halve B0 := ? (None, Any B0);
-buffer_halve (B1 a) := ? (Some a, Any B0);
-buffer_halve (B2 a b) := ? (None, Any (B1 (prodS a b)));
-buffer_halve (B3 a b c) := ? (Some a, Any (B1 (prodS b c)));
-buffer_halve (B4 a b c d) := ? (None, Any (B2 (prodS a b) (prodS c d)));
-buffer_halve (B5 a b c d e) := ? (Some a, Any (B2 (prodS b c) (prodS d e))).
+(* Makes a non-red buffer yellow. *)
+Equations to_yellow {A lvl g y} :
+  buffer A lvl (Mix g y NoRed) -> buffer A lvl yellow :=
+to_yellow (B1 a) := B1 a;
+to_yellow (B2 a b) := B2 a b;
+to_yellow (B3 a b c) := B3 a b c;
+to_yellow (B4 a b c d) := B4 a b c d.
 
-(* When [size1 = size2], translates a buffer of size1 to a buffer of size2. *)
+(* Proves the sequence of a buffer remains the same when it is made yellow. *)
+Lemma to_yellow_seq [A lvl g y] (b : buffer A lvl (Mix g y NoRed)) :
+  buffer_seq (to_yellow b) = buffer_seq b.
+Proof.
+  dependent destruction b; reflexivity.
+Qed.
 
-Equations buffer_translate {A lvl size1 size2 C} (b : buffer A lvl size1 C) :
-    size1 = size2 -> { b' : buffer A lvl size2 C | buffer_seq b' = buffer_seq b } :=
-buffer_translate b eq_refl := ? b.
+(* Makes a buffer of any color red. *)
+Equations to_red {A lvl C} : buffer A lvl C -> buffer A lvl red :=
+to_red B0 := B0;
+to_red (B1 a) := B1 a;
+to_red (B2 a b) := B2 a b;
+to_red (B3 a b c) := B3 a b c;
+to_red (B4 a b c d) := B4 a b c d;
+to_red (B5 a b c d e) := B5 a b c d e.
 
-(* A new tactic is introduced. It destructs every option and buffer in the
-   hypothesis. It is used to prove equality on sizes, by destructing options
-   and buffers, we are left with simple equations on natural numbers. *)
+(* Proves the sequence of a buffer remains the same when it is made red. *)
+Lemma to_red_seq [A lvl C] (b : buffer A lvl C) :
+  buffer_seq (to_red b) = buffer_seq b.
+Proof.
+  destruct b; reflexivity.
+Qed.
 
-Local Ltac destruct_opt_buff :=
-  do 7 (try match goal with
-  | o : option _ |- _ => destruct o
-  | b : buffer _ _ _ green |- _ => dependent destruction b
-  | b : buffer _ _ _ (Mix _ _ NoRed) |- _ => dependent destruction b
-  | b : buffer _ _ _ _ |- _ => dependent destruction b
-  end; cbn; try reflexivity).
+(* The last two lemmas are added to the hint database. *)
+#[export] Hint Rewrite to_yellow_seq : rlist.
+#[export] Hint Rewrite to_red_seq : rlist.
 
-#[local] Obligation Tactic :=
-  try first [ done | cbn; hauto db:rlist |
-  cbn beta iota; intros;
-  repeat match goal with H : _ = _ |- _ => clear H end;
-  destruct_opt_buff ].
+(* #[local] Obligation Tactic :=
+  try first [ cbn; hauto db:rlist ]. *)
 
-(* Takes any n-buffer and a green (n+1)-buffer, and rearranges elements
-   contained in the two buffers to return a green n-buffer and a yellow
-   (n+1)-buffer. The order of elements is preserved. *)
-
-Equations green_prefix_concat {A lvl size1 size2 C}
-  (buf1 : buffer A lvl size1 C)
-  (buf2 : buffer A (S lvl) size2 green) :
-  { '(buf1', buf2') : buffer A lvl (2 + size1 mod 2) green *
-                      yellow_buffer A (S lvl) (size2 - 1 + size1 / 2) |
-    buffer_seq buf1 ++ buffer_seq buf2 =
-    buffer_seq buf1' ++ yellow_buffer_seq buf2' } :=
-green_prefix_concat buf1 buf2 with prefix_decompose buf1 => {
-  | ? Ok buf with buffer_translate buf _, buffer_translate buf2 _ => {
-    | ? buf', ? buf2' := ? (buf', Yellowish buf2') };
-  | ? Underflow opt with green_pop buf2 => {
-    | ? (ab, Yellowish buf) with prefix23 opt ab => {
-      | ? prefix with buffer_translate prefix _, buffer_translate buf _ => {
-        | ? prefix', ? buf' := ? (prefix', Yellowish buf') } } };
-  | ? Overflow buf ab with buffer_translate buf _, green_push ab buf2 => {
-    | ? buf', ? suffix with buffer_translate suffix _ => {
-      | ? suffix' := ? (buf', Yellowish suffix') } } }.
-Next Obligation. Qed.
-
-(* Takes a green (n+1)-buffer and any n-buffer, and rearranges elements
-   contained in the two buffers to return a yellow (n+1)-buffer and a green
-   n-buffer. The order of elements is preserved. *)
-
-Equations green_suffix_concat {A lvl size1 size2 C}
-  (buf1 : buffer A (S lvl) size1 green)
-  (buf2 : buffer A lvl size2 C) :
-  { '(buf1', buf2') : yellow_buffer A (S lvl) (size1 - 1 + size2 / 2) *
-                      buffer A lvl (2 + size2 mod 2) green |
-    buffer_seq buf1 ++ buffer_seq buf2 =
-    yellow_buffer_seq buf1' ++ buffer_seq buf2' } :=
-green_suffix_concat buf1 buf2 with suffix_decompose buf2 => {
-  | ? Ok buf with buffer_translate buf1 _, buffer_translate buf _ => {
-    | ? buf1', ? buf' := ? (Yellowish buf1', buf') };
-  | ? Underflow opt with green_eject buf1 => {
-    | ? (Yellowish buf, ab) with suffix23 ab opt => {
-      | ? suffix with buffer_translate buf _, buffer_translate suffix _ => {
-      | ? buf', ? suffix' := ? (Yellowish buf', suffix') } } };
-  | ? Overflow buf ab with green_inject buf1 ab, buffer_translate buf _ => {
-    | ? prefix, ? buf' with buffer_translate prefix _ => {
-      | ? prefix' := ? (Yellowish prefix', buf') } } }.
-Next Obligation. Qed.
-
-(* Takes any n-buffer and a yellow (n+1)-buffer, and rearranges elements
-   contained in the two buffers to return a green n-buffer and any (n+1)-buffer.
+(* Takes a n-buffer of any color and a green (n+1)-buffer, rearranges elements
+   contained in them, and returns a green buffer and a yellow buffer of pairs.
    The order of elements is preserved. *)
+Equations green_prefix_concat {A lvl C}
+  (b1 : buffer A lvl C)
+  (b2 : buffer A (S lvl) green) :
+  { '(b1', b2') : buffer A lvl green * buffer A (S lvl) yellow |
+    buffer_seq b1 ++ buffer_seq b2 =
+    buffer_seq b1' ++ buffer_seq b2' } :=
+green_prefix_concat b1 b2 with prefix_decompose b1 => {
+  | ? Underflow opt with green_pop b2 => {
+    | ? (ab, b) with prefix23 opt ab => {
+      | ? prefix := ? (prefix, b) } };
+  | ? Ok b => ? (b, to_yellow b2);
+  | ? Overflow b ab with green_push ab b2 => {
+    | ? suffix := ? (b, suffix) } }.
 
-Equations yellow_prefix_concat {A lvl size1 size2 C}
-  (buf1 : buffer A lvl size1 C)
-  (buf2 : yellow_buffer A (S lvl) size2) :
-  { '(buf1', buf2') : buffer A lvl (2 + size1 mod 2) green *
-                      any_buffer A (S lvl) (size2 - 1 + size1 / 2) |
-    buffer_seq buf1 ++ yellow_buffer_seq buf2 =
-    buffer_seq buf1' ++ any_buffer_seq buf2' } :=
-yellow_prefix_concat buf1 (Yellowish buf2) with prefix_decompose buf1 => {
-  | ? Ok buf with buffer_translate buf _, buffer_translate buf2 _ => {
-    | ? buf', ? buf2' := ? (buf', Any buf2') };
-  | ? Underflow opt with yellow_pop (Yellowish buf2) => {
-    | ? (ab, Any buf) with prefix23 opt ab => {
-      | ? prefix with buffer_translate prefix _, buffer_translate buf _ => {
-        | ? prefix', ? buf' := ? (prefix', Any buf') } } };
-  | ? Overflow buf ab with buffer_translate buf _, yellow_push ab (Yellowish buf2) => {
-    | ? buf', ? Any suffix with buffer_translate suffix _ => {
-      | ? suffix' := ? (buf', Any suffix') } } }.
-Next Obligation. Qed.
-
-(* Takes a yellow (n+1)-buffer and any n-buffer, and rearranges elements
-   contained in the two buffers to return any (n+1)-buffer and a green n-buffer.
+(* Takes a green (n+1)-buffer and a n-buffer of any color, rearranges elements
+   contained in them, and returns a yellow buffer of pairs and a green buffer.
    The order of elements is preserved. *)
+Equations green_suffix_concat {A lvl C}
+  (b1 : buffer A (S lvl) green)
+  (b2 : buffer A lvl C) :
+  { '(b1', b2') : buffer A (S lvl) yellow * buffer A lvl green |
+    buffer_seq b1 ++ buffer_seq b2 =
+    buffer_seq b1' ++ buffer_seq b2' } :=
+green_suffix_concat b1 b2 with suffix_decompose b2 => {
+  | ? Underflow opt with green_eject b1 => {
+    | ? (b, ab) with suffix23 ab opt => {
+      | ? suffix := ? (b, suffix) } };
+  | ? Ok b => ? (to_yellow b1, b);
+  | ? Overflow b ab with green_inject b1 ab => {
+    | ? prefix := ? (prefix, b) } }.
 
-Equations yellow_suffix_concat {A lvl size1 size2 C}
-  (buf1 : yellow_buffer A (S lvl) size1)
-  (buf2 : buffer A lvl size2 C) :
-  { '(buf1', buf2') : any_buffer A (S lvl) (size1 - 1 + size2 / 2) *
-                      buffer A lvl (2 + size2 mod 2) green |
-    yellow_buffer_seq buf1 ++ buffer_seq buf2 =
-    any_buffer_seq buf1' ++ buffer_seq buf2' } :=
-yellow_suffix_concat (Yellowish buf1) buf2 with suffix_decompose buf2 => {
-  | ? Ok buf with buffer_translate buf1 _, buffer_translate buf _ => {
-    | ? buf1', ? buf' := ? (Any buf1', buf') };
-  | ? Underflow opt with yellow_eject (Yellowish buf1) => {
-    | ? (Any buf, ab) with suffix23 ab opt => {
-      | ? suffix with buffer_translate buf _, buffer_translate suffix _ => {
-        | ? buf', ? suffix' := ? (Any buf', suffix') } } };
-  | ? Overflow buf ab with yellow_inject (Yellowish buf1) ab, buffer_translate buf _ => {
-    | ? Any prefix, ? buf' with buffer_translate prefix _ => {
-      | ? prefix' := ? (Any prefix', buf') } } }.
-Next Obligation. Qed.
+(* Takes a n-buffer of any color and a yellow (n+1)-buffer, rearranges elements
+   contained in them, and returns a green buffer and a buffer of pairs of any
+   color.
+   The order of elements is preserved. *)
+Equations yellow_prefix_concat {A lvl C}
+  (b1 : buffer A lvl C)
+  (b2 : buffer A (S lvl) yellow) :
+  { '(b1', b2') : buffer A lvl green * buffer A (S lvl) red |
+    buffer_seq b1 ++ buffer_seq b2 =
+    buffer_seq b1' ++ buffer_seq b2' } :=
+yellow_prefix_concat b1 b2 with prefix_decompose b1 => {
+  | ? Underflow opt with yellow_pop b2 => {
+    | ? (ab, b) with prefix23 opt ab => {
+      | ? prefix := ? (prefix, b) } };
+  | ? Ok b => ? (b, to_red b2);
+  | ? Overflow b ab with yellow_push ab b2 => {
+    | ? suffix := ? (b, suffix) } }.
 
-(* Creates a green colored deque from three options, two of level n and one of
-   level n+1. *)
+(* Takes a yellow (n+1)-buffer and a n-buffer of any color, rearranges elements
+   contained in them, and returns a buffer of pairs of any color and a green
+   buffer.
+   The order of elements is preserved. *)
+Equations yellow_suffix_concat {A lvl C}
+  (b1 : buffer A (S lvl) yellow)
+  (b2 : buffer A lvl C) :
+  { '(b1', b2') : buffer A (S lvl) red * buffer A lvl green |
+    buffer_seq b1 ++ buffer_seq b2 =
+    buffer_seq b1' ++ buffer_seq b2' } :=
+yellow_suffix_concat b1 b2 with suffix_decompose b2 => {
+  | ? Underflow opt with yellow_eject b1 => {
+    | ? (b, ab) with suffix23 ab opt => {
+      | ? suffix := ? (b, suffix) } };
+  | ? Ok b => ? (to_red b1, b);
+  | ? Overflow b ab with yellow_inject b1 ab => {
+    | ? prefix := ? (prefix, b) } }.
 
-Equations cdeque_of_opt3 {A lvl}
-  (o1 : option (prodN A lvl))
-  (o2 : option (prodN A (S lvl)))
-  (o3 : option (prodN A lvl)) :
-  { cd : cdeque A lvl (size_option o1 + size_option o2 +
-                       size_option o2 + size_option o3) green |
-    cdeque_seq cd = option_seq o1 ++ option_seq o2 ++ option_seq o3 } :=
-cdeque_of_opt3 None None None := ? Small B0;
-cdeque_of_opt3 (Some a) None None := ? Small (B1 a);
-cdeque_of_opt3 None None (Some a) := ? Small (B1 a);
-cdeque_of_opt3 (Some a) None (Some b) := ? Small (B2 a b);
-cdeque_of_opt3 None (Some (prodS a b)) None := ? Small (B2 a b);
-cdeque_of_opt3 (Some a) (Some (prodS b c)) None := ? Small (B3 a b c);
-cdeque_of_opt3 None (Some (prodS a b)) (Some c) := ? Small (B3 a b c);
-cdeque_of_opt3 (Some a) (Some (prodS b c)) (Some d) := ? Small (B4 a b c d).
+(* Creates a green chain from 3 options. *)
+Equations chain_of_opt3 {A lvl}
+  (o1 : optionN A lvl) (o2 : optionN A (S lvl)) (o3 : optionN A lvl) :
+  { c : chain A lvl green |
+    chain_seq c = optionN_seq o1 ++ optionN_seq o2 ++ optionN_seq o3 } :=
+chain_of_opt3 None None None := ? Ending B0;
+chain_of_opt3 (Some a) None None := ? Ending (B1 a);
+chain_of_opt3 None None (Some a) := ? Ending (B1 a);
+chain_of_opt3 (Some a) None (Some b) := ? Ending (B2 a b);
+chain_of_opt3 None (Some (prodS a b)) None := ? Ending (B2 a b);
+chain_of_opt3 (Some a) (Some (prodS b c)) None := ? Ending (B3 a b c);
+chain_of_opt3 None (Some (prodS a b)) (Some c) := ? Ending (B3 a b c);
+chain_of_opt3 (Some a) (Some (prodS b c)) (Some d) := ? Ending (B4 a b c d).
 
-(* When [size1 = size2], translates a colored deque of size1 to a colored
-   deque of size2. *)
-
-Equations cdeque_translate {A lvl size1 size2 C} (cd : cdeque A lvl size1 C) :
-    size1 = size2 -> { cd' : cdeque A lvl size2 C | cdeque_seq cd' = cdeque_seq cd } :=
-cdeque_translate cd eq_refl := ? cd.
-
-(* A new tactic [destruct_prod] is introduced. It destructs all elements of
-   higher level into elements of lower levels. *)
-
-Local Ltac destruct_prod :=
-  repeat
-  match goal with
-  | a : prodN _ 0 |- _ => dependent destruction a
-  | ab : prodN _ (S _) |- _ => dependent destruction ab
-  | p : _ * _ |- _ => destruct p
-  end; cbn in *.
-
-(* A new tactic [to_size] is introduced. It converts an equality on lists to
-   an equality on their sizes. *)
-
-Local Ltac to_size H :=
-  apply (f_equal (@length _)) in H;
-  repeat rewrite app_length in H;
-  repeat rewrite buffer_size in H;
-  repeat rewrite prodN_size in H;
-  repeat rewrite option_size in H;
-  repeat rewrite deque_size in H.
-
-(* Small lemmas needed for the next tactics. *)
-
-Lemma add_r {n m p : nat} : n + p = m + p -> n = m.
-Proof. lia. Qed.
-
-Lemma add_r_0 {m p : nat} : p = m + p -> 0 = m.
-Proof. lia. Qed.
-
-Lemma add_l_0 {n p : nat} : n + p = p -> n = 0.
-Proof. lia. Qed.
-
-(* A new tactic [absurd_power2_eq] is introduced. It aims at showing that an
-   equality of sums of powers of 2 is wrong. *)
-
-Local Ltac absurd_power2_eq :=
-  repeat
-  match goal with
-  | H : 0 = power2 _ + _ |- _ =>
-    exfalso; symmetry in H;
-    apply Nat.eq_add_0 in H as [H1 H2]; apply (power2_neq0 H1)
-  | H : _ + power2 _ = 0 |- _ =>
-    exfalso; apply Nat.eq_add_0 in H as [H1 H2]; apply (power2_neq0 H2)
-  | H : _ + power2 ?n = _ + power2 ?n |- _ => apply add_r in H
-  | H : power2 ?n = _ + power2 ?n |- _ => apply add_r_0 in H
-  | H : _ + power2 ?n = power2 ?n |- _ => apply add_l_0 in H
-  end.
-
-#[local] Hint Rewrite Nat.add_assoc : rnat.
-#[local] Hint Rewrite Nat.add_0_r : rnat.
-
-#[local] Obligation Tactic :=
-  try first [ done | cbn; destruct_prod; hauto db:rlist ];
-  cbn beta iota match; intros.
-
-(* Takes a prefix buffer, a following buffer (when the next level is composed
-   of only one buffer), and a suffix buffer. It allows to rearrange all
-   elements contained in those buffers into a green cdeque. *)
-
-Equations make_small {A lvl size1 size2 size3 C1 C2 C3}
-  (b1 : buffer A lvl size1 C1)
-  (b2 : buffer A (S lvl) size2 C2)
-  (b3 : buffer A lvl size3 C3) :
-  { cd : cdeque A lvl (size1 + size2 + size2 + size3) green |
-    cdeque_seq cd = buffer_seq b1 ++ buffer_seq b2 ++ buffer_seq b3 } :=
-make_small prefix1 buf suffix1
-  with prefix_decompose prefix1, suffix_decompose suffix1 => {
-  | ? Underflow p1, ? Underflow s1 with buffer_unsandwich buf => {
-    | ? Alone opt2 with cdeque_of_opt3 p1 opt2 s1 => { | ? cd := ? cd };
+(* Takes a prefix buffer, a child buffer, and a suffix buffer, and rearranges
+   all elements contained in these buffers to form a green chain.
+   The order of elements is preserved. *)
+Equations make_small {A lvl C1 C2 C3}
+  (b1 : buffer A lvl C1)
+  (b2 : buffer A (S lvl) C2)
+  (b3 : buffer A lvl C3) :
+  { cd : chain A lvl green |
+    chain_seq cd = buffer_seq b1 ++ buffer_seq b2 ++ buffer_seq b3 } :=
+make_small b1 b2 b3 with (prefix_decompose b1), (suffix_decompose b3) => {
+  | ? Underflow p1, ? Underflow s1 with buffer_unsandwich b2 => {
+    | ? Alone opt with chain_of_opt3 p1 opt s1 => { | ? c := ? c };
     | ? Sandwich ab rest cd with prefix23 p1 ab, suffix23 cd s1 => {
-      | ? prefix, ? suffix :=
-      ? Big (Triple prefix Hole suffix PCGreen) (Small rest) eq_refl _ CCGreen } };
-  | ? Underflow None, ? Ok s1 with buffer_pop buf => {
-    | ? None with cdeque_translate (Small s1) _ => { | ? cd := ? cd };
-    | ? Some (prodS c d, Any rest) :=
-      ? Big (Triple (B2 c d) Hole s1 PCGreen) (Small rest) eq_refl _ CCGreen };
-  | ? Underflow (Some a), ? Ok s1 with buffer_pop buf => {
-    | ? None with buffer_push a s1 => {
-      | ? cd with cdeque_translate cd _ => { | ? cd' := ? cd' } };
-    | ? Some (prodS c d, Any rest) :=
-      ? Big (Triple (B3 a c d) Hole s1 PCGreen) (Small rest) eq_refl _ CCGreen };
-  | ? Underflow opt, ? Overflow s1 ab with suffix_rot buf ab => {
-    | ? (p', rest) with prefix23 opt p' => {
-      | ? prefix =>
-        ? Big (Triple prefix Hole s1 PCGreen) (Small rest) eq_refl _ CCGreen } };
-  | ? Ok p1, ? Underflow None with buffer_eject buf => {
-    | ? None with cdeque_translate (Small p1) _ => { | ? cd := ? cd };
-    | ? Some (Any rest, prodS c d) :=
-        ? Big (Triple p1 Hole (B2 c d) PCGreen) (Small rest) eq_refl _ CCGreen };
-  | ? Ok p1, ? Underflow (Some a) with buffer_eject buf => {
-  | ? None with buffer_inject p1 a => {
-      | ? cd with cdeque_translate cd _ => { | ? cd' := ? cd' } };
-  | ? Some (Any rest, prodS c d) :=
-      ? Big (Triple p1 Hole (B3 c d a) PCGreen) (Small rest) eq_refl _ CCGreen };
-  | ? Ok p1, ? Ok s1 :=
-    ? Big (Triple p1 Hole s1 PCGreen) (Small buf) eq_refl _ CCGreen;
-  | ? Ok p1, ? Overflow (size := size3') s1 ab with buffer_inject buf ab => {
-    | ? cd := ? Big (Triple p1 Hole s1 PCGreen) cd eq_refl _ CCGreen };
-  | ? Overflow p1 ab, ? Underflow opt with prefix_rot ab buf => {
-    | ? (rest, p') with suffix23 p' opt => {
-      | ? suffix =>
-        ? Big (Triple p1 Hole suffix PCGreen) (Small rest) eq_refl _ CCGreen } };
-  | ? Overflow p1 ab, ? Ok s1 with buffer_push ab buf => {
-    | ? cd := ? Big (Triple p1 Hole s1 PCGreen) cd eq_refl _ CCGreen };
-  | ? Overflow p1 ab, ? Overflow s1 cd with buffer_halve buf => {
-    | ? (x, Any rest) with suffix12 ab x => {
-      | ? prefix => ?
-        Big (Triple p1 (Triple prefix Hole (B1 cd) PCYellow) s1 PCGreen)
-            (Small rest) eq_refl _ CCGreen } } }.
+      | ? p, ? s := ? Chain G (Packet p Hole s) (Ending rest) } };
+  | ? Underflow p1, ? Ok s1 with buffer_pop b2 => {
+    | ? None with p1 => {
+      | None := ? Ending (to_red s1);
+      | Some x with buffer_push x s1 => { | ? c := ? c } };
+    | ? Some (cd, rest) with prefix23 p1 cd => {
+      | ? p := ? Chain G (Packet p Hole s1) (Ending rest) } };
+  | ? Underflow p1, ? Overflow s1 ab with suffix_rot b2 ab => {
+    | ? (cd, center) with prefix23 p1 cd => {
+      | ? p => ? Chain G (Packet p Hole s1) (Ending (to_red center)) } };
+  | ? Ok p1, ? Underflow s1 with buffer_eject b2 => {
+    | ? None with s1 => {
+      | None := ? Ending (to_red p1);
+      | Some x with buffer_inject p1 x => { | ? c := ? c } };
+    | ? Some (rest, ab) with suffix23 ab s1 => {
+      | ? s := ? Chain G (Packet p1 Hole s) (Ending rest) } };
+  | ? Ok p1, ? Ok s1 := ? Chain G (Packet p1 Hole s1) (Ending (to_red b2));
+  | ? Ok p1, ? Overflow s1 ab with buffer_inject b2 ab => {
+    | ? c2 => ? Chain G (Packet p1 Hole s1) c2 };
+  | ? Overflow p1 cd, ? Underflow s1 with prefix_rot cd b2 => {
+    | ? (center, ab) with suffix23 ab s1 => {
+      | ? s => ? Chain G (Packet p1 Hole s) (Ending (to_red center)) } };
+  | ? Overflow p1 cd, ? Ok s1 with buffer_push cd b2 => {
+    | ? c2 => ? Chain G (Packet p1 Hole s1) c2 };
+  | ? Overflow p1 cd, ? Overflow s1 ab with buffer_halve b2 => {
+    | ? (x, rest) with prefix12 cd x => {
+      | ? p =>
+        ? Chain G (Packet p1 (Packet p Hole (B1 ab)) s1) (Ending rest) } } }.
 Next Obligation.
-  to_size e1; destruct_opt_buff; simpl in e1; rewrite Nat.add_0_r in e1;
-  absurd_power2_eq.
+  cbn beta iota. intros * Hb1 * Hp * Hb2 Hb3. cbn.
+  rewrite to_red_seq, Hp.
+  aac_rewrite <-Hb2.
+  hauto db:rlist.
 Qed.
 Next Obligation.
-  apply empty_buffer_size in e1; subst; reflexivity.
-Qed.
-Next Obligation.
-  to_size e1; destruct_opt_buff; simpl in e1; rewrite Nat.add_0_r in e1;
-  absurd_power2_eq.
-Qed.
-Next Obligation.
-  apply empty_buffer_size in e1; subst; reflexivity.
-Qed.
-Next Obligation.
-  simp cdeque_seq packet_left_seq packet_right_seq;
-  destruct_prod; rewrite e1; aac_rewrite <-y; hauto db:rlist.
-Qed.
-Next Obligation.
-  to_size e1; destruct_opt_buff; simpl in e1; absurd_power2_eq.
-Qed.
-Next Obligation.
-  apply empty_buffer_size in e1; subst; lia.
-Qed.
-Next Obligation.
-  to_size e1; destruct_opt_buff; simpl in e1; absurd_power2_eq.
-Qed.
-Next Obligation.
-  apply empty_buffer_size in e1; subst; lia.
-Qed.
-Next Obligation.
-  simp cdeque_seq packet_left_seq packet_right_seq;
-  destruct_prod; rewrite e1; aac_rewrite <-y; hauto db:rlist.
-Qed.
-Next Obligation.
-  to_size y; destruct_opt_buff; simp size_option in y;
-  simpl in y; autorewrite with rnat in y; absurd_power2_eq.
+  cbn beta iota. intros * Hb1 * Hb2 * Hs Hb3. cbn.
+  rewrite to_red_seq, Hs.
+  aac_rewrite <-Hb2.
+  hauto db:rlist.
 Qed.
 
-(* Takes a red cdeque and returns a green one representing the same set. *)
-
-Equations green_of_red {A lvl size} (cd : cdeque A lvl size red) :
-  { cd' : cdeque A lvl size green | cdeque_seq cd' = cdeque_seq cd } :=
-green_of_red (Big (Triple p1 Hole s1 PCRed) (Small buf) eq_refl eq_refl CCRed)
-  with make_small p1 buf s1 => {
-    | ? cd with cdeque_translate cd _ => { | ? cd' := ? cd' } };
-green_of_red
-  (Big (Triple p1 (Triple p2 child s2 PCYellow) s1 PCRed) cd eq_refl eq_refl CCRed)
-    with yellow_prefix_concat p1 (Yellowish p2),
-         yellow_suffix_concat (Yellowish s2) s1 => {
-      | ? (p1', Any p2'), ? (Any s2', s1') :=
-        ? Big (Triple p1' Hole s1' PCGreen)
-              (Big (Triple p2' child s2' PCRed) cd _  eq_refl CCRed) _ _ CCGreen };
-green_of_red
-  (Big (Triple p1 Hole s1 PCRed)
-       (Big (Triple p2 child s2 PCGreen)
-            cd eq_refl eq_refl CCGreen) eq_refl eq_refl CCRed)
+(* Makes a red chain green. *)
+Equations green_of_red {A lvl} (cd : chain A lvl red) :
+  { cd' : chain A lvl green | chain_seq cd' = chain_seq cd } :=
+green_of_red (Chain R (Packet p1 Hole s1) (Ending b))
+  with make_small p1 b s1 => { | ? c' := ? c' };
+green_of_red (Chain R (Packet p1 Hole s1) (Chain G (Packet p2 child s2) c))
   with green_prefix_concat p1 p2, green_suffix_concat s2 s1 => {
-    | ? (p1', Yellowish p2'), ? (Yellowish s2', s1') :=
-    ? Big (Triple p1' (Triple p2' child s2' PCYellow) s1' PCGreen) cd _ _ CCGreen }.
+  | ? (p1', p2'), ? (s2', s1') :=
+    ? Chain G (Packet p1' (Packet p2' child s2') s1') c };
+green_of_red (Chain R (Packet p1 (Packet p2 child s2) s1) c)
+  with yellow_prefix_concat p1 (to_yellow p2),
+       yellow_suffix_concat (to_yellow s2) s1 => {
+  | ? (p1', p2'), ? (s2', s1') :=
+    ? Chain G (Packet p1' Hole s1') (Chain R (Packet p2' child s2') c) }.
 Next Obligation.
-  dependent destruction p1; dependent destruction s1;
-  (match goal with
-  | b : buffer _ _ psize0 _ |- _ =>
-    dependent destruction b end);
-  dependent destruction s2; simpl; lia.
+  cbn. intros * Hp * Hs *.
+  aac_rewrite <-Hp.
+  hauto db:rlist.
 Qed.
 Next Obligation.
-  simp cdeque_seq packet_left_seq packet_right_seq;
-  autorewrite with rlist;
-  simp yellow_buffer_seq in y, y0;
-  aac_rewrite <-y; aac_normalise;
-  do 5 apply <-app_inv_head_iff;
-  symmetry; assumption.
-Qed.
-Next Obligation.
-  dependent destruction p1; dependent destruction s1;
-  (match goal with
-  | b : buffer _ _ psize0 _ |- _ =>
-    dependent destruction b end);
-  dependent destruction s2; simpl; lia.
-Qed.
-Next Obligation.
-  simp cdeque_seq packet_left_seq packet_right_seq;
-  autorewrite with rlist;
-  simp yellow_buffer_seq any_buffer_seq in y, y0;
-  aac_rewrite <-y; aac_normalise;
-  do 5 apply <-app_inv_head_iff;
-  symmetry; assumption.
+  cbn. intros * Hp * Hs *.
+  aac_rewrite <-Hp.
+  hauto db:rlist.
 Qed.
 
-(* Takes a green or red cdeque, and returns a green one representing
-   the same set. *)
+(* Makes a green or red chain green. *)
+Equations ensure_green {A lvl G R} (cd : chain A lvl (Mix G NoYellow R)) :
+  { cd' : chain A lvl green | chain_seq cd' = chain_seq cd } :=
+ensure_green (Ending b)      := ? Ending b;
+ensure_green (Chain G pkt c) := ? Chain G pkt c;
+ensure_green (Chain R pkt c) := green_of_red (Chain R pkt c).
 
-Equations ensure_green {A lvl size G R}
-  (cd : cdeque A lvl size (Mix G NoYellow R)) :
-  { cd' : cdeque A lvl size green | cdeque_seq cd' = cdeque_seq cd } :=
-ensure_green (Small buf) := ? Small buf;
-ensure_green (Big x cd eq_refl eq_refl CCGreen) := ? Big x cd _ eq_refl CCGreen;
-ensure_green (Big x cd eq_refl eq_refl CCRed) :=
-  green_of_red (Big x cd _ eq_refl CCRed).
+(* Takes a prefix non-red buffer, a child packet and a suffix non-red buffer,
+   and a following green or red chain, and makes a deque out of them. *)
+Equations make_yellow {A hlvl g1 y1 y2 g3 y3 g4 r4}
+  (p : buffer A 0 (Mix g1 y1 NoRed))
+  (pkt : packet A 1 hlvl (Mix NoGreen y2 NoRed))
+  (s : buffer A 0 (Mix g3 y3 NoRed))
+  (c : chain A hlvl (Mix g4 NoYellow r4)) :
+  { d : deque A | deque_seq d =
+    buffer_seq p ++ packet_seq pkt (chain_seq c) ++ buffer_seq s } :=
+make_yellow p1 child s1 c with ensure_green c => {
+  | ? c' => ? T (Chain Y (Packet (to_yellow p1) child (to_yellow s1)) c') }.
 
-(* Takes a yellow packet, as a prefix buffer, a child packet and a suffix
-   buffer, and a green or red cdeque. Returns a deque starting with this packet
-   and followed by the green version of the input colored deque. *)
+(* Takes a prefix buffer of any color, a child packet and a suffix buffer of
+   any color, and a following green chain, and makes a deque out of them. *)
+Equations make_red {A hlvl C1 y2 C3}
+  (p : buffer A 0 C1)
+  (pkt : packet A 1 hlvl (Mix NoGreen y2 NoRed))
+  (s : buffer A 0 C3)
+  (c : chain A hlvl green) :
+  { d : deque A | deque_seq d =
+    buffer_seq p ++ packet_seq pkt (chain_seq c) ++ buffer_seq s } :=
+make_red p1 child s1 c
+  with green_of_red (Chain R (Packet (to_red p1) child (to_red s1)) c) => {
+    | ? c' => ? T c' }.
 
-Equations make_yellow {A len size1 pktsize size2 cdsize} {G1 Y1 Y2 G3 Y3 G4 R4}
-  (buf1 : buffer A 0 size1 (Mix G1 Y1 NoRed))
-  (p : packet A 1 len pktsize (Mix NoGreen Y2 NoRed))
-  (buf2 : buffer A 0 size2 (Mix G3 Y3 NoRed))
-  (cd : cdeque A (S len + 0) cdsize (Mix G4 NoYellow R4)) :
-  { d : deque A (size1 + pktsize + pktsize + size2 + (power2 (S len)) * cdsize) |
-    deque_seq d = buffer_seq buf1 ++
-                   packet_left_seq p ++
-                   cdeque_seq cd ++
-                   packet_right_seq p ++
-                   buffer_seq buf2 } :=
-make_yellow p1 child s1 cd with ensure_green cd => {
-  | ? cd' => ? T (Big (Triple p1 child s1 PCYellow) cd' _ eq_refl CCYellow) }.
+(* +------------------------------------------------------------------------+ *)
+(* |                               Operations                               | *)
+(* +------------------------------------------------------------------------+ *)
 
-(* Takes a red packet, as a prefix buffer, a child packet and a suffix
-   buffer, and a green cdeque. Returns the green version of the colored deque
-   made of the red packet followed by the green cdeque. *)
+(* Pushes on a deque. *)
+Equations push {A: Type} (x : A) (d : deque A) :
+  { d' : deque A | deque_seq d' = [x] ++ deque_seq d } :=
+push x (T (Ending b)) with buffer_push (prodZ x) b => { | ? b' => ? T b' };
+push x (T (Chain G (Packet p1 child s1) c))
+  with green_push (prodZ x) p1 => {
+    | ? p1' with make_yellow p1' child s1 c => { | ? d' => ? d' } };
+push x (T (Chain Y (Packet p1 child s1) c))
+  with yellow_push (prodZ x) p1 => {
+    | ? p1' with make_red p1' child s1 c => { | ? d' => ? d' } }.
 
-Equations make_red {A len size1 pktsize size2 cdsize} {C1 Y2 C3}
-  (buf1 : buffer A 0 size1 C1)
-  (p : packet A 1 len pktsize (Mix NoGreen Y2 NoRed))
-  (buf2 : buffer A 0 size2 C3)
-  (cd : cdeque A (S len + 0) cdsize green) :
-  { d : deque A (size1 + pktsize + pktsize + size2 + (power2 (S len)) * cdsize) |
-    deque_seq d = buffer_seq buf1 ++
-                  packet_left_seq p ++
-                  cdeque_seq cd ++
-                  packet_right_seq p ++
-                  buffer_seq buf2 } :=
-make_red p1 child s1 cd
-  with green_of_red (Big (Triple p1 child s1 PCRed) cd _ eq_refl CCRed) => {
-    | ? cd' => ? T cd' }.
+(* Injects on a deque. *)
+Equations inject {A: Type} (d : deque A) (x : A) :
+  { d' : deque A | deque_seq d' = deque_seq d ++ [x] } :=
+inject (T (Ending b)) x with buffer_inject b (prodZ x) => { | ? b' => ? T b' };
+inject (T (Chain G (Packet p1 child s1) c)) x
+  with green_inject s1 (prodZ x) => {
+    | ? s1' with make_yellow p1 child s1' c => { | ? d' => ? d' } };
+inject (T (Chain Y (Packet p1 child s1) c)) x
+  with yellow_inject s1 (prodZ x) => {
+    | ? s1' with make_red p1 child s1' c => { | ? d' => ? d' } }.
 
-(* When [size1 = size2], translates a deque of size1 to a deque of size2. *)
-
-Equations deque_translate {A size1 size2} (d : deque A size1) :
-    size1 = size2 -> { d' : deque A size2 | deque_seq d' = deque_seq d } :=
-deque_translate d eq_refl := ? d.
-
-#[local] Obligation Tactic :=
-  try first [
-    done |
-    cbn; destruct_prod; hauto db:rlist |
-    cbn; intros; destruct_opt_buff; lia ];
-  cbn beta iota match; intros.
-
-(* Pushes an element on a deque. *)
-
-Equations push {A size} (x : A) (d : deque A size) :
-  { d' : deque A (S size) | deque_seq d' = [x] ++ deque_seq d } :=
-push x (T (Small buf)) with buffer_push (prodZ x) buf => {
-  | ? buf' => ? T buf' };
-push x (T (Big (Triple p1 child s1 PCGreen) dq eq_refl eq_refl CCGreen)) with green_push (prodZ x) p1 => {
-  | ? buf' with make_yellow buf' child s1 dq => {
-    | ? d' => ? d' } };
-push x (T (Big (Triple p1 child s1 PCYellow) dq eq_refl eq_refl CCYellow))
-  with yellow_push (prodZ x) (Yellowish p1) => {
-  | ? (Any p1') with make_red p1' child s1 dq => {
-    | ? d' => ? d' } }.
-
-(* Injects an element on a deque. *)
-
-Equations inject {A size} (d : deque A size) (x : A) :
-  { d' : deque A (S size) | deque_seq d' = deque_seq d ++ [x] } :=
-inject (T (Small buf)) x with buffer_inject buf (prodZ x) => {
-  | ? buf' => ? T buf' };
-inject (T (Big (Triple p1 child s1 PCGreen) cd eq_refl eq_refl CCGreen)) x with green_inject s1 (prodZ x) => {
-  | ? buf' with make_yellow p1 child buf' cd => {
-    | ? d' with deque_translate d' _ => { | ? d'' := ? d'' } } };
-inject (T (Big (Triple p1 child s1 PCYellow) cd eq_refl eq_refl CCYellow)) x
-  with yellow_inject (Yellowish s1) (prodZ x) => {
-  | ? (Any s1') with make_red p1 child s1' cd => {
-    | ? d' with deque_translate d' _ => { | ? d'' := ? d'' } } }.
-
-(* Pops an element from a deque. *)
-
-Equations unsafe_pop {A size} (d : deque A size) :
-  { o : option (A * deque A (Nat.pred size)) |
+(* Pops off a deque. *)
+Equations pop {A: Type} (d : deque A) :
+  { o : option (A * deque A) |
     deque_seq d = match o with
-               | None => []
-               | Some (x, d') => [x] ++ deque_seq d'
-               end } :=
-unsafe_pop (T (Small buf)) with buffer_pop buf => {
+                  | None => []
+                  | Some (x, d') => [x] ++ deque_seq d'
+                  end } :=
+pop (T (Ending b)) with buffer_pop b => {
   | ? None := ? None;
-  | ? Some (prodZ x, Any buf') := ? Some (x, T (Small buf'))
-};
-unsafe_pop (T (Big (Triple p1 child s1 PCGreen) cd eq_refl eq_refl CCGreen)) with green_pop p1 => {
-  | ? (prodZ x, Yellowish p1') with make_yellow p1' child s1 cd => {
-    | ? d' with deque_translate d' _ => { | ? d'' := ? Some (x, d'') } } };
-unsafe_pop (T (Big (Triple p1 child s1 PCYellow) cd eq_refl eq_refl CCYellow)) with yellow_pop (Yellowish p1) => {
-  | ? (prodZ x, Any p1') with make_red p1' child s1 cd => {
-    | ? d' with deque_translate d' _ => { | ? d'' := ? Some (x, d'') } } }.
+  | ? Some (prodZ x, b') := ? Some (x, T (Ending b')) };
+pop (T (Chain G (Packet p1 child s1) c)) with green_pop p1 => {
+  | ? (prodZ x, p1') with make_yellow p1' child s1 c => {
+    | ? d' => ? Some (x, d') } };
+pop (T (Chain Y (Packet p1 child s1) c)) with yellow_pop p1 => {
+  | ? (prodZ x, p1') with make_red p1' child s1 c => {
+    | ? d' => ? Some (x, d') } }.
 
-Equations pop {A size} (d : deque A (S size)) :
-  { '(x, d') : A * deque A size | [x] ++ deque_seq d' = deque_seq d } :=
-pop d with unsafe_pop d => {
-  | ? None := _;
-  | ? Some (x, d') := ? (x, d') }.
-Next Obligation.
-  to_size e; apply Nat.neq_succ_0 in e; destruct e.
-Qed.
-
-(* Ejects an element from a deque. *)
-
-Equations unsafe_eject {A size} (d : deque A size) :
-  { o : option (deque A (Nat.pred size) * A) |
+(* Ejects off a deque. *)
+Equations eject {A : Type} (d : deque A) :
+  { o : option (deque A * A) |
     deque_seq d = match o with
-               | None => []
-               | Some (d', x) => deque_seq d' ++ [x]
-               end } :=
-unsafe_eject (T (Small buf)) with buffer_eject buf => {
+                  | None => []
+                  | Some (d', x) => deque_seq d' ++ [x]
+                  end } :=
+eject (T (Ending b)) with buffer_eject b => {
   | ? None := ? None;
-  | ? Some (Any buf', prodZ x) := ? Some (T (Small buf'), x)
-};
-unsafe_eject (T (Big (Triple p1 child s1 PCGreen) cd eq_refl eq_refl CCGreen)) with green_eject s1 => {
-  | ? (Yellowish s1', prodZ x) with make_yellow p1 child s1' cd => {
-    | ? d' with deque_translate d' _ => { | ? d'' := ? Some (d'', x) } } };
-unsafe_eject (T (Big (Triple p1 child s1 PCYellow) cd eq_refl eq_refl CCYellow)) with yellow_eject (Yellowish s1) => {
-  | ? (Any s1', prodZ x) with make_red p1 child s1' cd => {
-    | ? d' with deque_translate d' _ => { | ? d'' := ? Some (d'', x) } } }.
-
-Equations eject {A size} (d : deque A (S size)) :
-  { '(d', x) : deque A size * A | deque_seq d' ++ [x] = deque_seq d } :=
-eject d with unsafe_eject d => {
-  | ? None := _;
-  | ? Some (d', x) := ? (d', x) }.
-Next Obligation.
-  to_size e; apply Nat.neq_succ_0 in e; destruct e.
-Qed.
+  | ? Some (b', prodZ x) := ? Some (T (Ending b'), x) };
+eject (T (Chain G (Packet p1 child s1) c)) with green_eject s1 => {
+  | ? (s1',prodZ  x) with make_yellow p1 child s1' c => {
+    | ? d' => ? Some (d', x) } };
+eject (T (Chain Y (Packet p1 child s1) c)) with yellow_eject s1 => {
+  | ? (s1', prodZ x) with make_red p1 child s1' c => {
+    | ? d' => ? Some (d', x) } }.
